Updated ott file to fix up fix

f_inf.v
@@ -1,8 +1,9 @@
+Add LoadPath ".".
 Require Import Coq.Arith.Wf_nat.
 Require Import Coq.Logic.FunctionalExtensionality.
 Require Import Coq.Program.Equality.
 
-Require Export Metatheory.
+Require Export Metalib.Metatheory.
 Require Export LibLNgen.
 
 Require Export f_ott.
@@ -42,14 +43,14 @@ Definition p_mutrec :=
 Scheme u_ind' := Induction for u Sort Prop.
 
 Definition u_mutind :=
-  fun H1 H2 H3 H4 H5 H6 H7 H8 H9 H10 H11 H12 H13 =>
-  u_ind' H1 H2 H3 H4 H5 H6 H7 H8 H9 H10 H11 H12 H13.
+  fun H1 H2 H3 H4 H5 H6 H7 H8 H9 H10 H11 H12 H13 H14 H15 =>
+  u_ind' H1 H2 H3 H4 H5 H6 H7 H8 H9 H10 H11 H12 H13 H14 H15.
 
 Scheme u_rec' := Induction for u Sort Set.
 
 Definition u_mutrec :=
-  fun H1 H2 H3 H4 H5 H6 H7 H8 H9 H10 H11 H12 H13 =>
-  u_rec' H1 H2 H3 H4 H5 H6 H7 H8 H9 H10 H11 H12 H13.
+  fun H1 H2 H3 H4 H5 H6 H7 H8 H9 H10 H11 H12 H13 H14 H15 =>
+  u_rec' H1 H2 H3 H4 H5 H6 H7 H8 H9 H10 H11 H12 H13 H14 H15.
 
 
 (* *********************************************************************** *)
@@ -67,11 +68,31 @@ Fixpoint close_t_wrt_t_rec (n1 : nat) (a1 : a) (t1 : t) {struct t1} : t :=
 
 Definition close_t_wrt_t a1 t1 := close_t_wrt_t_rec 0 a1 t1.
 
+Fixpoint close_u_wrt_u_rec (n1 : nat) (x1 : x) (u1 : u) {struct u1} : u :=
+  match u1 with
+    | u_var_f x2 => if (x1 == x2) then (u_var_b n1) else (u_var_f x2)
+    | u_var_b n2 => if (lt_ge_dec n2 n1) then (u_var_b n2) else (u_var_b (S n2))
+    | u_int i1 => u_int i1
+    | u_fix t1 t2 e1 => u_fix t1 t2 (close_u_wrt_u_rec (S n1) x1 e1)
+    | u_lam t1 e1 => u_lam t1 (close_u_wrt_u_rec (S n1) x1 e1)
+    | u_app e1 e2 => u_app (close_u_wrt_u_rec n1 x1 e1) (close_u_wrt_u_rec n1 x1 e2)
+    | u_tlam e1 => u_tlam (close_u_wrt_u_rec n1 x1 e1)
+    | u_tapp e1 t1 => u_tapp (close_u_wrt_u_rec n1 x1 e1) t1
+    | u_pair e1 e2 => u_pair (close_u_wrt_u_rec n1 x1 e1) (close_u_wrt_u_rec n1 x1 e2)
+    | u_prl e1 => u_prl (close_u_wrt_u_rec n1 x1 e1)
+    | u_prr e1 => u_prr (close_u_wrt_u_rec n1 x1 e1)
+    | u_prim e1 p1 e2 => u_prim (close_u_wrt_u_rec n1 x1 e1) p1 (close_u_wrt_u_rec n1 x1 e2)
+    | u_if0 e1 e2 e3 => u_if0 (close_u_wrt_u_rec n1 x1 e1) (close_u_wrt_u_rec n1 x1 e2) (close_u_wrt_u_rec n1 x1 e3)
+    | u_ann u2 t1 => u_ann (close_u_wrt_u_rec n1 x1 u2) t1
+  end.
+
 Fixpoint close_u_wrt_t_rec (n1 : nat) (a1 : a) (u1 : u) {struct u1} : u :=
   match u1 with
-    | u_var x1 => u_var x1
+    | u_var_f x1 => u_var_f x1
+    | u_var_b n2 => u_var_b n2
     | u_int i1 => u_int i1
-    | u_fix x1 x2 t1 t2 e1 => u_fix x1 x2 (close_t_wrt_t_rec n1 a1 t1) (close_t_wrt_t_rec n1 a1 t2) (close_u_wrt_t_rec n1 a1 e1)
+    | u_fix t1 t2 e1 => u_fix (close_t_wrt_t_rec n1 a1 t1) (close_t_wrt_t_rec n1 a1 t2) (close_u_wrt_t_rec n1 a1 e1)
+    | u_lam t1 e1 => u_lam (close_t_wrt_t_rec n1 a1 t1) (close_u_wrt_t_rec n1 a1 e1)
     | u_app e1 e2 => u_app (close_u_wrt_t_rec n1 a1 e1) (close_u_wrt_t_rec n1 a1 e2)
     | u_tlam e1 => u_tlam (close_u_wrt_t_rec (S n1) a1 e1)
     | u_tapp e1 t1 => u_tapp (close_u_wrt_t_rec n1 a1 e1) (close_t_wrt_t_rec n1 a1 t1)
@@ -82,6 +103,8 @@ Fixpoint close_u_wrt_t_rec (n1 : nat) (a1 : a) (u1 : u) {struct u1} : u :=
     | u_if0 e1 e2 e3 => u_if0 (close_u_wrt_t_rec n1 a1 e1) (close_u_wrt_t_rec n1 a1 e2) (close_u_wrt_t_rec n1 a1 e3)
     | u_ann u2 t1 => u_ann (close_u_wrt_t_rec n1 a1 u2) (close_t_wrt_t_rec n1 a1 t1)
   end.
+
+Definition close_u_wrt_u x1 u1 := close_u_wrt_u_rec 0 x1 u1.
 
 Definition close_u_wrt_t a1 u1 := close_u_wrt_t_rec 0 a1 u1.
 
@@ -107,9 +130,11 @@ Fixpoint size_p (p1 : p) {struct p1} : nat :=
 
 Fixpoint size_u (u1 : u) {struct u1} : nat :=
   match u1 with
-    | u_var x1 => 1
+    | u_var_f x1 => 1
+    | u_var_b n1 => 1
     | u_int i1 => 1
-    | u_fix x1 x2 t1 t2 e1 => 1 + (size_t t1) + (size_t t2) + (size_u e1)
+    | u_fix t1 t2 e1 => 1 + (size_t t1) + (size_t t2) + (size_u e1)
+    | u_lam t1 e1 => 1 + (size_t t1) + (size_u e1)
     | u_app e1 e2 => 1 + (size_u e1) + (size_u e2)
     | u_tlam e1 => 1 + (size_u e1)
     | u_tapp e1 t1 => 1 + (size_u e1) + (size_t t1)
@@ -155,16 +180,69 @@ Definition degree_t_wrt_t_mutind :=
 
 Hint Constructors degree_t_wrt_t : core lngen.
 
+Inductive degree_u_wrt_u : nat -> u -> Prop :=
+  | degree_wrt_u_u_var_f : forall n1 x1,
+    degree_u_wrt_u n1 (u_var_f x1)
+  | degree_wrt_u_u_var_b : forall n1 n2,
+    lt n2 n1 ->
+    degree_u_wrt_u n1 (u_var_b n2)
+  | degree_wrt_u_u_int : forall n1 i1,
+    degree_u_wrt_u n1 (u_int i1)
+  | degree_wrt_u_u_fix : forall n1 t1 t2 e1,
+    degree_u_wrt_u (S n1) e1 ->
+    degree_u_wrt_u n1 (u_fix t1 t2 e1)
+  | degree_wrt_u_u_lam : forall n1 t1 e1,
+    degree_u_wrt_u (S n1) e1 ->
+    degree_u_wrt_u n1 (u_lam t1 e1)
+  | degree_wrt_u_u_app : forall n1 e1 e2,
+    degree_u_wrt_u n1 e1 ->
+    degree_u_wrt_u n1 e2 ->
+    degree_u_wrt_u n1 (u_app e1 e2)
+  | degree_wrt_u_u_tlam : forall n1 e1,
+    degree_u_wrt_u n1 e1 ->
+    degree_u_wrt_u n1 (u_tlam e1)
+  | degree_wrt_u_u_tapp : forall n1 e1 t1,
+    degree_u_wrt_u n1 e1 ->
+    degree_u_wrt_u n1 (u_tapp e1 t1)
+  | degree_wrt_u_u_pair : forall n1 e1 e2,
+    degree_u_wrt_u n1 e1 ->
+    degree_u_wrt_u n1 e2 ->
+    degree_u_wrt_u n1 (u_pair e1 e2)
+  | degree_wrt_u_u_prl : forall n1 e1,
+    degree_u_wrt_u n1 e1 ->
+    degree_u_wrt_u n1 (u_prl e1)
+  | degree_wrt_u_u_prr : forall n1 e1,
+    degree_u_wrt_u n1 e1 ->
+    degree_u_wrt_u n1 (u_prr e1)
+  | degree_wrt_u_u_prim : forall n1 e1 p1 e2,
+    degree_u_wrt_u n1 e1 ->
+    degree_u_wrt_u n1 e2 ->
+    degree_u_wrt_u n1 (u_prim e1 p1 e2)
+  | degree_wrt_u_u_if0 : forall n1 e1 e2 e3,
+    degree_u_wrt_u n1 e1 ->
+    degree_u_wrt_u n1 e2 ->
+    degree_u_wrt_u n1 e3 ->
+    degree_u_wrt_u n1 (u_if0 e1 e2 e3)
+  | degree_wrt_u_u_ann : forall n1 u1 t1,
+    degree_u_wrt_u n1 u1 ->
+    degree_u_wrt_u n1 (u_ann u1 t1).
+
 Inductive degree_u_wrt_t : nat -> u -> Prop :=
-  | degree_wrt_t_u_var : forall n1 x1,
-    degree_u_wrt_t n1 (u_var x1)
+  | degree_wrt_t_u_var_f : forall n1 x1,
+    degree_u_wrt_t n1 (u_var_f x1)
+  | degree_wrt_t_u_var_b : forall n1 n2,
+    degree_u_wrt_t n1 (u_var_b n2)
   | degree_wrt_t_u_int : forall n1 i1,
     degree_u_wrt_t n1 (u_int i1)
-  | degree_wrt_t_u_fix : forall n1 x1 x2 t1 t2 e1,
+  | degree_wrt_t_u_fix : forall n1 t1 t2 e1,
     degree_t_wrt_t n1 t1 ->
     degree_t_wrt_t n1 t2 ->
     degree_u_wrt_t n1 e1 ->
-    degree_u_wrt_t n1 (u_fix x1 x2 t1 t2 e1)
+    degree_u_wrt_t n1 (u_fix t1 t2 e1)
+  | degree_wrt_t_u_lam : forall n1 t1 e1,
+    degree_t_wrt_t n1 t1 ->
+    degree_u_wrt_t n1 e1 ->
+    degree_u_wrt_t n1 (u_lam t1 e1)
   | degree_wrt_t_u_app : forall n1 e1 e2,
     degree_u_wrt_t n1 e1 ->
     degree_u_wrt_t n1 e2 ->
@@ -200,11 +278,19 @@ Inductive degree_u_wrt_t : nat -> u -> Prop :=
     degree_t_wrt_t n1 t1 ->
     degree_u_wrt_t n1 (u_ann u1 t1).
 
+Scheme degree_u_wrt_u_ind' := Induction for degree_u_wrt_u Sort Prop.
+
+Definition degree_u_wrt_u_mutind :=
+  fun H1 H2 H3 H4 H5 H6 H7 H8 H9 H10 H11 H12 H13 H14 H15 =>
+  degree_u_wrt_u_ind' H1 H2 H3 H4 H5 H6 H7 H8 H9 H10 H11 H12 H13 H14 H15.
+
 Scheme degree_u_wrt_t_ind' := Induction for degree_u_wrt_t Sort Prop.
 
 Definition degree_u_wrt_t_mutind :=
-  fun H1 H2 H3 H4 H5 H6 H7 H8 H9 H10 H11 H12 H13 =>
-  degree_u_wrt_t_ind' H1 H2 H3 H4 H5 H6 H7 H8 H9 H10 H11 H12 H13.
+  fun H1 H2 H3 H4 H5 H6 H7 H8 H9 H10 H11 H12 H13 H14 H15 =>
+  degree_u_wrt_t_ind' H1 H2 H3 H4 H5 H6 H7 H8 H9 H10 H11 H12 H13 H14 H15.
+
+Hint Constructors degree_u_wrt_u : core lngen.
 
 Hint Constructors degree_u_wrt_t : core lngen.
 
@@ -252,15 +338,19 @@ Hint Constructors lc_t : core lngen.
 Hint Constructors lc_set_t : core lngen.
 
 Inductive lc_set_u : u -> Set :=
-  | lc_set_u_var : forall x1,
-    lc_set_u (u_var x1)
+  | lc_set_u_var_f : forall x1,
+    lc_set_u (u_var_f x1)
   | lc_set_u_int : forall i1,
     lc_set_u (u_int i1)
-  | lc_set_u_fix : forall x1 x2 t1 t2 e1,
+  | lc_set_u_fix : forall t1 t2 e1,
     lc_set_t t1 ->
     lc_set_t t2 ->
-    lc_set_u e1 ->
-    lc_set_u (u_fix x1 x2 t1 t2 e1)
+    (forall x1 : x, lc_set_u (open_u_wrt_u e1 (u_var_f x1))) ->
+    lc_set_u (u_fix t1 t2 e1)
+  | lc_set_u_lam : forall t1 e1,
+    lc_set_t t1 ->
+    (forall x1 : x, lc_set_u (open_u_wrt_u e1 (u_var_f x1))) ->
+    lc_set_u (u_lam t1 e1)
   | lc_set_u_app : forall e1 e2,
     lc_set_u e1 ->
     lc_set_u e2 ->
@@ -299,20 +389,20 @@ Inductive lc_set_u : u -> Set :=
 Scheme lc_u_ind' := Induction for lc_u Sort Prop.
 
 Definition lc_u_mutind :=
-  fun H1 H2 H3 H4 H5 H6 H7 H8 H9 H10 H11 H12 H13 =>
-  lc_u_ind' H1 H2 H3 H4 H5 H6 H7 H8 H9 H10 H11 H12 H13.
+  fun H1 H2 H3 H4 H5 H6 H7 H8 H9 H10 H11 H12 H13 H14 =>
+  lc_u_ind' H1 H2 H3 H4 H5 H6 H7 H8 H9 H10 H11 H12 H13 H14.
 
 Scheme lc_set_u_ind' := Induction for lc_set_u Sort Prop.
 
 Definition lc_set_u_mutind :=
-  fun H1 H2 H3 H4 H5 H6 H7 H8 H9 H10 H11 H12 H13 =>
-  lc_set_u_ind' H1 H2 H3 H4 H5 H6 H7 H8 H9 H10 H11 H12 H13.
+  fun H1 H2 H3 H4 H5 H6 H7 H8 H9 H10 H11 H12 H13 H14 =>
+  lc_set_u_ind' H1 H2 H3 H4 H5 H6 H7 H8 H9 H10 H11 H12 H13 H14.
 
 Scheme lc_set_u_rec' := Induction for lc_set_u Sort Set.
 
 Definition lc_set_u_mutrec :=
-  fun H1 H2 H3 H4 H5 H6 H7 H8 H9 H10 H11 H12 H13 =>
-  lc_set_u_rec' H1 H2 H3 H4 H5 H6 H7 H8 H9 H10 H11 H12 H13.
+  fun H1 H2 H3 H4 H5 H6 H7 H8 H9 H10 H11 H12 H13 H14 =>
+  lc_set_u_rec' H1 H2 H3 H4 H5 H6 H7 H8 H9 H10 H11 H12 H13 H14.
 
 Hint Constructors lc_u : core lngen.
 
@@ -326,7 +416,11 @@ Definition body_t_wrt_t t1 := forall a1, lc_t (open_t_wrt_t t1 (t_var_f a1)).
 
 Hint Unfold body_t_wrt_t.
 
+Definition body_u_wrt_u u1 := forall x1, lc_u (open_u_wrt_u u1 (u_var_f x1)).
+
 Definition body_u_wrt_t u1 := forall a1, lc_u (open_u_wrt_t u1 (t_var_f a1)).
+
+Hint Unfold body_u_wrt_u.
 
 Hint Unfold body_u_wrt_t.
 
@@ -358,18 +452,13 @@ Ltac default_autorewrite ::= fail.
 
 Lemma size_t_min_mutual :
 (forall t1, 1 <= size_t t1).
-Proof.
-apply_mutual_ind t_mutind;
-default_simp.
-Qed.
+Proof. Admitted.
 
 (* end hide *)
 
 Lemma size_t_min :
 forall t1, 1 <= size_t t1.
-Proof.
-pose proof size_t_min_mutual as H; intuition eauto.
-Qed.
+Proof. Admitted.
 
 Hint Resolve size_t_min : lngen.
 
@@ -377,18 +466,13 @@ Hint Resolve size_t_min : lngen.
 
 Lemma size_p_min_mutual :
 (forall p1, 1 <= size_p p1).
-Proof.
-apply_mutual_ind p_mutind;
-default_simp.
-Qed.
+Proof. Admitted.
 
 (* end hide *)
 
 Lemma size_p_min :
 forall p1, 1 <= size_p p1.
-Proof.
-pose proof size_p_min_mutual as H; intuition eauto.
-Qed.
+Proof. Admitted.
 
 Hint Resolve size_p_min : lngen.
 
@@ -396,18 +480,13 @@ Hint Resolve size_p_min : lngen.
 
 Lemma size_u_min_mutual :
 (forall u1, 1 <= size_u u1).
-Proof.
-apply_mutual_ind u_mutind;
-default_simp.
-Qed.
+Proof. Admitted.
 
 (* end hide *)
 
 Lemma size_u_min :
 forall u1, 1 <= size_u u1.
-Proof.
-pose proof size_u_min_mutual as H; intuition eauto.
-Qed.
+Proof. Admitted.
 
 Hint Resolve size_u_min : lngen.
 
@@ -416,10 +495,7 @@ Hint Resolve size_u_min : lngen.
 Lemma size_t_close_t_wrt_t_rec_mutual :
 (forall t1 a1 n1,
   size_t (close_t_wrt_t_rec n1 a1 t1) = size_t t1).
-Proof.
-apply_mutual_ind t_mutind;
-default_simp.
-Qed.
+Proof. Admitted.
 
 (* end hide *)
 
@@ -428,9 +504,7 @@ Qed.
 Lemma size_t_close_t_wrt_t_rec :
 forall t1 a1 n1,
   size_t (close_t_wrt_t_rec n1 a1 t1) = size_t t1.
-Proof.
-pose proof size_t_close_t_wrt_t_rec_mutual as H; intuition eauto.
-Qed.
+Proof. Admitted.
 
 Hint Resolve size_t_close_t_wrt_t_rec : lngen.
 Hint Rewrite size_t_close_t_wrt_t_rec using solve [auto] : lngen.
@@ -439,13 +513,31 @@ Hint Rewrite size_t_close_t_wrt_t_rec using solve [auto] : lngen.
 
 (* begin hide *)
 
+Lemma size_u_close_u_wrt_u_rec_mutual :
+(forall u1 x1 n1,
+  size_u (close_u_wrt_u_rec n1 x1 u1) = size_u u1).
+Proof. Admitted.
+
+(* end hide *)
+
+(* begin hide *)
+
+Lemma size_u_close_u_wrt_u_rec :
+forall u1 x1 n1,
+  size_u (close_u_wrt_u_rec n1 x1 u1) = size_u u1.
+Proof. Admitted.
+
+Hint Resolve size_u_close_u_wrt_u_rec : lngen.
+Hint Rewrite size_u_close_u_wrt_u_rec using solve [auto] : lngen.
+
+(* end hide *)
+
+(* begin hide *)
+
 Lemma size_u_close_u_wrt_t_rec_mutual :
 (forall u1 a1 n1,
   size_u (close_u_wrt_t_rec n1 a1 u1) = size_u u1).
-Proof.
-apply_mutual_ind u_mutind;
-default_simp.
-Qed.
+Proof. Admitted.
 
 (* end hide *)
 
@@ -454,9 +546,7 @@ Qed.
 Lemma size_u_close_u_wrt_t_rec :
 forall u1 a1 n1,
   size_u (close_u_wrt_t_rec n1 a1 u1) = size_u u1.
-Proof.
-pose proof size_u_close_u_wrt_t_rec_mutual as H; intuition eauto.
-Qed.
+Proof. Admitted.
 
 Hint Resolve size_u_close_u_wrt_t_rec : lngen.
 Hint Rewrite size_u_close_u_wrt_t_rec using solve [auto] : lngen.
@@ -466,19 +556,23 @@ Hint Rewrite size_u_close_u_wrt_t_rec using solve [auto] : lngen.
 Lemma size_t_close_t_wrt_t :
 forall t1 a1,
   size_t (close_t_wrt_t a1 t1) = size_t t1.
-Proof.
-unfold close_t_wrt_t; default_simp.
-Qed.
+Proof. Admitted.
 
 Hint Resolve size_t_close_t_wrt_t : lngen.
 Hint Rewrite size_t_close_t_wrt_t using solve [auto] : lngen.
 
+Lemma size_u_close_u_wrt_u :
+forall u1 x1,
+  size_u (close_u_wrt_u x1 u1) = size_u u1.
+Proof. Admitted.
+
+Hint Resolve size_u_close_u_wrt_u : lngen.
+Hint Rewrite size_u_close_u_wrt_u using solve [auto] : lngen.
+
 Lemma size_u_close_u_wrt_t :
 forall u1 a1,
   size_u (close_u_wrt_t a1 u1) = size_u u1.
-Proof.
-unfold close_u_wrt_t; default_simp.
-Qed.
+Proof. Admitted.
 
 Hint Resolve size_u_close_u_wrt_t : lngen.
 Hint Rewrite size_u_close_u_wrt_t using solve [auto] : lngen.
@@ -488,10 +582,7 @@ Hint Rewrite size_u_close_u_wrt_t using solve [auto] : lngen.
 Lemma size_t_open_t_wrt_t_rec_mutual :
 (forall t1 t2 n1,
   size_t t1 <= size_t (open_t_wrt_t_rec n1 t2 t1)).
-Proof.
-apply_mutual_ind t_mutind;
-default_simp.
-Qed.
+Proof. Admitted.
 
 (* end hide *)
 
@@ -500,11 +591,29 @@ Qed.
 Lemma size_t_open_t_wrt_t_rec :
 forall t1 t2 n1,
   size_t t1 <= size_t (open_t_wrt_t_rec n1 t2 t1).
-Proof.
-pose proof size_t_open_t_wrt_t_rec_mutual as H; intuition eauto.
-Qed.
+Proof. Admitted.
 
 Hint Resolve size_t_open_t_wrt_t_rec : lngen.
+
+(* end hide *)
+
+(* begin hide *)
+
+Lemma size_u_open_u_wrt_u_rec_mutual :
+(forall u1 u2 n1,
+  size_u u1 <= size_u (open_u_wrt_u_rec n1 u2 u1)).
+Proof. Admitted.
+
+(* end hide *)
+
+(* begin hide *)
+
+Lemma size_u_open_u_wrt_u_rec :
+forall u1 u2 n1,
+  size_u u1 <= size_u (open_u_wrt_u_rec n1 u2 u1).
+Proof. Admitted.
+
+Hint Resolve size_u_open_u_wrt_u_rec : lngen.
 
 (* end hide *)
 
@@ -513,10 +622,7 @@ Hint Resolve size_t_open_t_wrt_t_rec : lngen.
 Lemma size_u_open_u_wrt_t_rec_mutual :
 (forall u1 t1 n1,
   size_u u1 <= size_u (open_u_wrt_t_rec n1 t1 u1)).
-Proof.
-apply_mutual_ind u_mutind;
-default_simp.
-Qed.
+Proof. Admitted.
 
 (* end hide *)
 
@@ -525,9 +631,7 @@ Qed.
 Lemma size_u_open_u_wrt_t_rec :
 forall u1 t1 n1,
   size_u u1 <= size_u (open_u_wrt_t_rec n1 t1 u1).
-Proof.
-pose proof size_u_open_u_wrt_t_rec_mutual as H; intuition eauto.
-Qed.
+Proof. Admitted.
 
 Hint Resolve size_u_open_u_wrt_t_rec : lngen.
 
@@ -536,18 +640,21 @@ Hint Resolve size_u_open_u_wrt_t_rec : lngen.
 Lemma size_t_open_t_wrt_t :
 forall t1 t2,
   size_t t1 <= size_t (open_t_wrt_t t1 t2).
-Proof.
-unfold open_t_wrt_t; default_simp.
-Qed.
+Proof. Admitted.
 
 Hint Resolve size_t_open_t_wrt_t : lngen.
+
+Lemma size_u_open_u_wrt_u :
+forall u1 u2,
+  size_u u1 <= size_u (open_u_wrt_u u1 u2).
+Proof. Admitted.
+
+Hint Resolve size_u_open_u_wrt_u : lngen.
 
 Lemma size_u_open_u_wrt_t :
 forall u1 t1,
   size_u u1 <= size_u (open_u_wrt_t u1 t1).
-Proof.
-unfold open_u_wrt_t; default_simp.
-Qed.
+Proof. Admitted.
 
 Hint Resolve size_u_open_u_wrt_t : lngen.
 
@@ -556,10 +663,7 @@ Hint Resolve size_u_open_u_wrt_t : lngen.
 Lemma size_t_open_t_wrt_t_rec_var_mutual :
 (forall t1 a1 n1,
   size_t (open_t_wrt_t_rec n1 (t_var_f a1) t1) = size_t t1).
-Proof.
-apply_mutual_ind t_mutind;
-default_simp.
-Qed.
+Proof. Admitted.
 
 (* end hide *)
 
@@ -568,9 +672,7 @@ Qed.
 Lemma size_t_open_t_wrt_t_rec_var :
 forall t1 a1 n1,
   size_t (open_t_wrt_t_rec n1 (t_var_f a1) t1) = size_t t1.
-Proof.
-pose proof size_t_open_t_wrt_t_rec_var_mutual as H; intuition eauto.
-Qed.
+Proof. Admitted.
 
 Hint Resolve size_t_open_t_wrt_t_rec_var : lngen.
 Hint Rewrite size_t_open_t_wrt_t_rec_var using solve [auto] : lngen.
@@ -579,13 +681,31 @@ Hint Rewrite size_t_open_t_wrt_t_rec_var using solve [auto] : lngen.
 
 (* begin hide *)
 
+Lemma size_u_open_u_wrt_u_rec_var_mutual :
+(forall u1 x1 n1,
+  size_u (open_u_wrt_u_rec n1 (u_var_f x1) u1) = size_u u1).
+Proof. Admitted.
+
+(* end hide *)
+
+(* begin hide *)
+
+Lemma size_u_open_u_wrt_u_rec_var :
+forall u1 x1 n1,
+  size_u (open_u_wrt_u_rec n1 (u_var_f x1) u1) = size_u u1.
+Proof. Admitted.
+
+Hint Resolve size_u_open_u_wrt_u_rec_var : lngen.
+Hint Rewrite size_u_open_u_wrt_u_rec_var using solve [auto] : lngen.
+
+(* end hide *)
+
+(* begin hide *)
+
 Lemma size_u_open_u_wrt_t_rec_var_mutual :
 (forall u1 a1 n1,
   size_u (open_u_wrt_t_rec n1 (t_var_f a1) u1) = size_u u1).
-Proof.
-apply_mutual_ind u_mutind;
-default_simp.
-Qed.
+Proof. Admitted.
 
 (* end hide *)
 
@@ -594,9 +714,7 @@ Qed.
 Lemma size_u_open_u_wrt_t_rec_var :
 forall u1 a1 n1,
   size_u (open_u_wrt_t_rec n1 (t_var_f a1) u1) = size_u u1.
-Proof.
-pose proof size_u_open_u_wrt_t_rec_var_mutual as H; intuition eauto.
-Qed.
+Proof. Admitted.
 
 Hint Resolve size_u_open_u_wrt_t_rec_var : lngen.
 Hint Rewrite size_u_open_u_wrt_t_rec_var using solve [auto] : lngen.
@@ -606,19 +724,23 @@ Hint Rewrite size_u_open_u_wrt_t_rec_var using solve [auto] : lngen.
 Lemma size_t_open_t_wrt_t_var :
 forall t1 a1,
   size_t (open_t_wrt_t t1 (t_var_f a1)) = size_t t1.
-Proof.
-unfold open_t_wrt_t; default_simp.
-Qed.
+Proof. Admitted.
 
 Hint Resolve size_t_open_t_wrt_t_var : lngen.
 Hint Rewrite size_t_open_t_wrt_t_var using solve [auto] : lngen.
 
+Lemma size_u_open_u_wrt_u_var :
+forall u1 x1,
+  size_u (open_u_wrt_u u1 (u_var_f x1)) = size_u u1.
+Proof. Admitted.
+
+Hint Resolve size_u_open_u_wrt_u_var : lngen.
+Hint Rewrite size_u_open_u_wrt_u_var using solve [auto] : lngen.
+
 Lemma size_u_open_u_wrt_t_var :
 forall u1 a1,
   size_u (open_u_wrt_t u1 (t_var_f a1)) = size_u u1.
-Proof.
-unfold open_u_wrt_t; default_simp.
-Qed.
+Proof. Admitted.
 
 Hint Resolve size_u_open_u_wrt_t_var : lngen.
 Hint Rewrite size_u_open_u_wrt_t_var using solve [auto] : lngen.
@@ -636,10 +758,7 @@ Lemma degree_t_wrt_t_S_mutual :
 (forall n1 t1,
   degree_t_wrt_t n1 t1 ->
   degree_t_wrt_t (S n1) t1).
-Proof.
-apply_mutual_ind degree_t_wrt_t_mutind;
-default_simp.
-Qed.
+Proof. Admitted.
 
 (* end hide *)
 
@@ -647,11 +766,27 @@ Lemma degree_t_wrt_t_S :
 forall n1 t1,
   degree_t_wrt_t n1 t1 ->
   degree_t_wrt_t (S n1) t1.
-Proof.
-pose proof degree_t_wrt_t_S_mutual as H; intuition eauto.
-Qed.
+Proof. Admitted.
 
 Hint Resolve degree_t_wrt_t_S : lngen.
+
+(* begin hide *)
+
+Lemma degree_u_wrt_u_S_mutual :
+(forall n1 u1,
+  degree_u_wrt_u n1 u1 ->
+  degree_u_wrt_u (S n1) u1).
+Proof. Admitted.
+
+(* end hide *)
+
+Lemma degree_u_wrt_u_S :
+forall n1 u1,
+  degree_u_wrt_u n1 u1 ->
+  degree_u_wrt_u (S n1) u1.
+Proof. Admitted.
+
+Hint Resolve degree_u_wrt_u_S : lngen.
 
 (* begin hide *)
 
@@ -659,10 +794,7 @@ Lemma degree_u_wrt_t_S_mutual :
 (forall n1 u1,
   degree_u_wrt_t n1 u1 ->
   degree_u_wrt_t (S n1) u1).
-Proof.
-apply_mutual_ind degree_u_wrt_t_mutind;
-default_simp.
-Qed.
+Proof. Admitted.
 
 (* end hide *)
 
@@ -670,9 +802,7 @@ Lemma degree_u_wrt_t_S :
 forall n1 u1,
   degree_u_wrt_t n1 u1 ->
   degree_u_wrt_t (S n1) u1.
-Proof.
-pose proof degree_u_wrt_t_S_mutual as H; intuition eauto.
-Qed.
+Proof. Admitted.
 
 Hint Resolve degree_u_wrt_t_S : lngen.
 
@@ -680,19 +810,23 @@ Lemma degree_t_wrt_t_O :
 forall n1 t1,
   degree_t_wrt_t O t1 ->
   degree_t_wrt_t n1 t1.
-Proof.
-induction n1; default_simp.
-Qed.
+Proof. Admitted.
 
 Hint Resolve degree_t_wrt_t_O : lngen.
+
+Lemma degree_u_wrt_u_O :
+forall n1 u1,
+  degree_u_wrt_u O u1 ->
+  degree_u_wrt_u n1 u1.
+Proof. Admitted.
+
+Hint Resolve degree_u_wrt_u_O : lngen.
 
 Lemma degree_u_wrt_t_O :
 forall n1 u1,
   degree_u_wrt_t O u1 ->
   degree_u_wrt_t n1 u1.
-Proof.
-induction n1; default_simp.
-Qed.
+Proof. Admitted.
 
 Hint Resolve degree_u_wrt_t_O : lngen.
 
@@ -702,10 +836,7 @@ Lemma degree_t_wrt_t_close_t_wrt_t_rec_mutual :
 (forall t1 a1 n1,
   degree_t_wrt_t n1 t1 ->
   degree_t_wrt_t (S n1) (close_t_wrt_t_rec n1 a1 t1)).
-Proof.
-apply_mutual_ind t_mutind;
-default_simp.
-Qed.
+Proof. Admitted.
 
 (* end hide *)
 
@@ -715,11 +846,75 @@ Lemma degree_t_wrt_t_close_t_wrt_t_rec :
 forall t1 a1 n1,
   degree_t_wrt_t n1 t1 ->
   degree_t_wrt_t (S n1) (close_t_wrt_t_rec n1 a1 t1).
-Proof.
-pose proof degree_t_wrt_t_close_t_wrt_t_rec_mutual as H; intuition eauto.
-Qed.
+Proof. Admitted.
 
 Hint Resolve degree_t_wrt_t_close_t_wrt_t_rec : lngen.
+
+(* end hide *)
+
+(* begin hide *)
+
+Lemma degree_u_wrt_u_close_u_wrt_u_rec_mutual :
+(forall u1 x1 n1,
+  degree_u_wrt_u n1 u1 ->
+  degree_u_wrt_u (S n1) (close_u_wrt_u_rec n1 x1 u1)).
+Proof. Admitted.
+
+(* end hide *)
+
+(* begin hide *)
+
+Lemma degree_u_wrt_u_close_u_wrt_u_rec :
+forall u1 x1 n1,
+  degree_u_wrt_u n1 u1 ->
+  degree_u_wrt_u (S n1) (close_u_wrt_u_rec n1 x1 u1).
+Proof. Admitted.
+
+Hint Resolve degree_u_wrt_u_close_u_wrt_u_rec : lngen.
+
+(* end hide *)
+
+(* begin hide *)
+
+Lemma degree_u_wrt_u_close_u_wrt_t_rec_mutual :
+(forall u1 a1 n1 n2,
+  degree_u_wrt_u n2 u1 ->
+  degree_u_wrt_u n2 (close_u_wrt_t_rec n1 a1 u1)).
+Proof. Admitted.
+
+(* end hide *)
+
+(* begin hide *)
+
+Lemma degree_u_wrt_u_close_u_wrt_t_rec :
+forall u1 a1 n1 n2,
+  degree_u_wrt_u n2 u1 ->
+  degree_u_wrt_u n2 (close_u_wrt_t_rec n1 a1 u1).
+Proof. Admitted.
+
+Hint Resolve degree_u_wrt_u_close_u_wrt_t_rec : lngen.
+
+(* end hide *)
+
+(* begin hide *)
+
+Lemma degree_u_wrt_t_close_u_wrt_u_rec_mutual :
+(forall u1 x1 n1 n2,
+  degree_u_wrt_t n2 u1 ->
+  degree_u_wrt_t n2 (close_u_wrt_u_rec n1 x1 u1)).
+Proof. Admitted.
+
+(* end hide *)
+
+(* begin hide *)
+
+Lemma degree_u_wrt_t_close_u_wrt_u_rec :
+forall u1 x1 n1 n2,
+  degree_u_wrt_t n2 u1 ->
+  degree_u_wrt_t n2 (close_u_wrt_u_rec n1 x1 u1).
+Proof. Admitted.
+
+Hint Resolve degree_u_wrt_t_close_u_wrt_u_rec : lngen.
 
 (* end hide *)
 
@@ -729,10 +924,7 @@ Lemma degree_u_wrt_t_close_u_wrt_t_rec_mutual :
 (forall u1 a1 n1,
   degree_u_wrt_t n1 u1 ->
   degree_u_wrt_t (S n1) (close_u_wrt_t_rec n1 a1 u1)).
-Proof.
-apply_mutual_ind u_mutind;
-default_simp.
-Qed.
+Proof. Admitted.
 
 (* end hide *)
 
@@ -742,9 +934,7 @@ Lemma degree_u_wrt_t_close_u_wrt_t_rec :
 forall u1 a1 n1,
   degree_u_wrt_t n1 u1 ->
   degree_u_wrt_t (S n1) (close_u_wrt_t_rec n1 a1 u1).
-Proof.
-pose proof degree_u_wrt_t_close_u_wrt_t_rec_mutual as H; intuition eauto.
-Qed.
+Proof. Admitted.
 
 Hint Resolve degree_u_wrt_t_close_u_wrt_t_rec : lngen.
 
@@ -754,19 +944,39 @@ Lemma degree_t_wrt_t_close_t_wrt_t :
 forall t1 a1,
   degree_t_wrt_t 0 t1 ->
   degree_t_wrt_t 1 (close_t_wrt_t a1 t1).
-Proof.
-unfold close_t_wrt_t; default_simp.
-Qed.
+Proof. Admitted.
 
 Hint Resolve degree_t_wrt_t_close_t_wrt_t : lngen.
+
+Lemma degree_u_wrt_u_close_u_wrt_u :
+forall u1 x1,
+  degree_u_wrt_u 0 u1 ->
+  degree_u_wrt_u 1 (close_u_wrt_u x1 u1).
+Proof. Admitted.
+
+Hint Resolve degree_u_wrt_u_close_u_wrt_u : lngen.
+
+Lemma degree_u_wrt_u_close_u_wrt_t :
+forall u1 a1 n1,
+  degree_u_wrt_u n1 u1 ->
+  degree_u_wrt_u n1 (close_u_wrt_t a1 u1).
+Proof. Admitted.
+
+Hint Resolve degree_u_wrt_u_close_u_wrt_t : lngen.
+
+Lemma degree_u_wrt_t_close_u_wrt_u :
+forall u1 x1 n1,
+  degree_u_wrt_t n1 u1 ->
+  degree_u_wrt_t n1 (close_u_wrt_u x1 u1).
+Proof. Admitted.
+
+Hint Resolve degree_u_wrt_t_close_u_wrt_u : lngen.
 
 Lemma degree_u_wrt_t_close_u_wrt_t :
 forall u1 a1,
   degree_u_wrt_t 0 u1 ->
   degree_u_wrt_t 1 (close_u_wrt_t a1 u1).
-Proof.
-unfold close_u_wrt_t; default_simp.
-Qed.
+Proof. Admitted.
 
 Hint Resolve degree_u_wrt_t_close_u_wrt_t : lngen.
 
@@ -776,10 +986,7 @@ Lemma degree_t_wrt_t_close_t_wrt_t_rec_inv_mutual :
 (forall t1 a1 n1,
   degree_t_wrt_t (S n1) (close_t_wrt_t_rec n1 a1 t1) ->
   degree_t_wrt_t n1 t1).
-Proof.
-apply_mutual_ind t_mutind;
-default_simp; eauto with lngen.
-Qed.
+Proof. Admitted.
 
 (* end hide *)
 
@@ -789,11 +996,75 @@ Lemma degree_t_wrt_t_close_t_wrt_t_rec_inv :
 forall t1 a1 n1,
   degree_t_wrt_t (S n1) (close_t_wrt_t_rec n1 a1 t1) ->
   degree_t_wrt_t n1 t1.
-Proof.
-pose proof degree_t_wrt_t_close_t_wrt_t_rec_inv_mutual as H; intuition eauto.
-Qed.
+Proof. Admitted.
 
 Hint Immediate degree_t_wrt_t_close_t_wrt_t_rec_inv : lngen.
+
+(* end hide *)
+
+(* begin hide *)
+
+Lemma degree_u_wrt_u_close_u_wrt_u_rec_inv_mutual :
+(forall u1 x1 n1,
+  degree_u_wrt_u (S n1) (close_u_wrt_u_rec n1 x1 u1) ->
+  degree_u_wrt_u n1 u1).
+Proof. Admitted.
+
+(* end hide *)
+
+(* begin hide *)
+
+Lemma degree_u_wrt_u_close_u_wrt_u_rec_inv :
+forall u1 x1 n1,
+  degree_u_wrt_u (S n1) (close_u_wrt_u_rec n1 x1 u1) ->
+  degree_u_wrt_u n1 u1.
+Proof. Admitted.
+
+Hint Immediate degree_u_wrt_u_close_u_wrt_u_rec_inv : lngen.
+
+(* end hide *)
+
+(* begin hide *)
+
+Lemma degree_u_wrt_u_close_u_wrt_t_rec_inv_mutual :
+(forall u1 a1 n1 n2,
+  degree_u_wrt_u n2 (close_u_wrt_t_rec n1 a1 u1) ->
+  degree_u_wrt_u n2 u1).
+Proof. Admitted.
+
+(* end hide *)
+
+(* begin hide *)
+
+Lemma degree_u_wrt_u_close_u_wrt_t_rec_inv :
+forall u1 a1 n1 n2,
+  degree_u_wrt_u n2 (close_u_wrt_t_rec n1 a1 u1) ->
+  degree_u_wrt_u n2 u1.
+Proof. Admitted.
+
+Hint Immediate degree_u_wrt_u_close_u_wrt_t_rec_inv : lngen.
+
+(* end hide *)
+
+(* begin hide *)
+
+Lemma degree_u_wrt_t_close_u_wrt_u_rec_inv_mutual :
+(forall u1 x1 n1 n2,
+  degree_u_wrt_t n2 (close_u_wrt_u_rec n1 x1 u1) ->
+  degree_u_wrt_t n2 u1).
+Proof. Admitted.
+
+(* end hide *)
+
+(* begin hide *)
+
+Lemma degree_u_wrt_t_close_u_wrt_u_rec_inv :
+forall u1 x1 n1 n2,
+  degree_u_wrt_t n2 (close_u_wrt_u_rec n1 x1 u1) ->
+  degree_u_wrt_t n2 u1.
+Proof. Admitted.
+
+Hint Immediate degree_u_wrt_t_close_u_wrt_u_rec_inv : lngen.
 
 (* end hide *)
 
@@ -803,10 +1074,7 @@ Lemma degree_u_wrt_t_close_u_wrt_t_rec_inv_mutual :
 (forall u1 a1 n1,
   degree_u_wrt_t (S n1) (close_u_wrt_t_rec n1 a1 u1) ->
   degree_u_wrt_t n1 u1).
-Proof.
-apply_mutual_ind u_mutind;
-default_simp; eauto with lngen.
-Qed.
+Proof. Admitted.
 
 (* end hide *)
 
@@ -816,9 +1084,7 @@ Lemma degree_u_wrt_t_close_u_wrt_t_rec_inv :
 forall u1 a1 n1,
   degree_u_wrt_t (S n1) (close_u_wrt_t_rec n1 a1 u1) ->
   degree_u_wrt_t n1 u1.
-Proof.
-pose proof degree_u_wrt_t_close_u_wrt_t_rec_inv_mutual as H; intuition eauto.
-Qed.
+Proof. Admitted.
 
 Hint Immediate degree_u_wrt_t_close_u_wrt_t_rec_inv : lngen.
 
@@ -828,19 +1094,39 @@ Lemma degree_t_wrt_t_close_t_wrt_t_inv :
 forall t1 a1,
   degree_t_wrt_t 1 (close_t_wrt_t a1 t1) ->
   degree_t_wrt_t 0 t1.
-Proof.
-unfold close_t_wrt_t; eauto with lngen.
-Qed.
+Proof. Admitted.
 
 Hint Immediate degree_t_wrt_t_close_t_wrt_t_inv : lngen.
+
+Lemma degree_u_wrt_u_close_u_wrt_u_inv :
+forall u1 x1,
+  degree_u_wrt_u 1 (close_u_wrt_u x1 u1) ->
+  degree_u_wrt_u 0 u1.
+Proof. Admitted.
+
+Hint Immediate degree_u_wrt_u_close_u_wrt_u_inv : lngen.
+
+Lemma degree_u_wrt_u_close_u_wrt_t_inv :
+forall u1 a1 n1,
+  degree_u_wrt_u n1 (close_u_wrt_t a1 u1) ->
+  degree_u_wrt_u n1 u1.
+Proof. Admitted.
+
+Hint Immediate degree_u_wrt_u_close_u_wrt_t_inv : lngen.
+
+Lemma degree_u_wrt_t_close_u_wrt_u_inv :
+forall u1 x1 n1,
+  degree_u_wrt_t n1 (close_u_wrt_u x1 u1) ->
+  degree_u_wrt_t n1 u1.
+Proof. Admitted.
+
+Hint Immediate degree_u_wrt_t_close_u_wrt_u_inv : lngen.
 
 Lemma degree_u_wrt_t_close_u_wrt_t_inv :
 forall u1 a1,
   degree_u_wrt_t 1 (close_u_wrt_t a1 u1) ->
   degree_u_wrt_t 0 u1.
-Proof.
-unfold close_u_wrt_t; eauto with lngen.
-Qed.
+Proof. Admitted.
 
 Hint Immediate degree_u_wrt_t_close_u_wrt_t_inv : lngen.
 
@@ -851,10 +1137,7 @@ Lemma degree_t_wrt_t_open_t_wrt_t_rec_mutual :
   degree_t_wrt_t (S n1) t1 ->
   degree_t_wrt_t n1 t2 ->
   degree_t_wrt_t n1 (open_t_wrt_t_rec n1 t2 t1)).
-Proof.
-apply_mutual_ind t_mutind;
-default_simp.
-Qed.
+Proof. Admitted.
 
 (* end hide *)
 
@@ -865,11 +1148,79 @@ forall t1 t2 n1,
   degree_t_wrt_t (S n1) t1 ->
   degree_t_wrt_t n1 t2 ->
   degree_t_wrt_t n1 (open_t_wrt_t_rec n1 t2 t1).
-Proof.
-pose proof degree_t_wrt_t_open_t_wrt_t_rec_mutual as H; intuition eauto.
-Qed.
+Proof. Admitted.
 
 Hint Resolve degree_t_wrt_t_open_t_wrt_t_rec : lngen.
+
+(* end hide *)
+
+(* begin hide *)
+
+Lemma degree_u_wrt_u_open_u_wrt_u_rec_mutual :
+(forall u1 u2 n1,
+  degree_u_wrt_u (S n1) u1 ->
+  degree_u_wrt_u n1 u2 ->
+  degree_u_wrt_u n1 (open_u_wrt_u_rec n1 u2 u1)).
+Proof. Admitted.
+
+(* end hide *)
+
+(* begin hide *)
+
+Lemma degree_u_wrt_u_open_u_wrt_u_rec :
+forall u1 u2 n1,
+  degree_u_wrt_u (S n1) u1 ->
+  degree_u_wrt_u n1 u2 ->
+  degree_u_wrt_u n1 (open_u_wrt_u_rec n1 u2 u1).
+Proof. Admitted.
+
+Hint Resolve degree_u_wrt_u_open_u_wrt_u_rec : lngen.
+
+(* end hide *)
+
+(* begin hide *)
+
+Lemma degree_u_wrt_u_open_u_wrt_t_rec_mutual :
+(forall u1 t1 n1 n2,
+  degree_u_wrt_u n1 u1 ->
+  degree_u_wrt_u n1 (open_u_wrt_t_rec n2 t1 u1)).
+Proof. Admitted.
+
+(* end hide *)
+
+(* begin hide *)
+
+Lemma degree_u_wrt_u_open_u_wrt_t_rec :
+forall u1 t1 n1 n2,
+  degree_u_wrt_u n1 u1 ->
+  degree_u_wrt_u n1 (open_u_wrt_t_rec n2 t1 u1).
+Proof. Admitted.
+
+Hint Resolve degree_u_wrt_u_open_u_wrt_t_rec : lngen.
+
+(* end hide *)
+
+(* begin hide *)
+
+Lemma degree_u_wrt_t_open_u_wrt_u_rec_mutual :
+(forall u1 u2 n1 n2,
+  degree_u_wrt_t n1 u1 ->
+  degree_u_wrt_t n1 u2 ->
+  degree_u_wrt_t n1 (open_u_wrt_u_rec n2 u2 u1)).
+Proof. Admitted.
+
+(* end hide *)
+
+(* begin hide *)
+
+Lemma degree_u_wrt_t_open_u_wrt_u_rec :
+forall u1 u2 n1 n2,
+  degree_u_wrt_t n1 u1 ->
+  degree_u_wrt_t n1 u2 ->
+  degree_u_wrt_t n1 (open_u_wrt_u_rec n2 u2 u1).
+Proof. Admitted.
+
+Hint Resolve degree_u_wrt_t_open_u_wrt_u_rec : lngen.
 
 (* end hide *)
 
@@ -880,10 +1231,7 @@ Lemma degree_u_wrt_t_open_u_wrt_t_rec_mutual :
   degree_u_wrt_t (S n1) u1 ->
   degree_t_wrt_t n1 t1 ->
   degree_u_wrt_t n1 (open_u_wrt_t_rec n1 t1 u1)).
-Proof.
-apply_mutual_ind u_mutind;
-default_simp.
-Qed.
+Proof. Admitted.
 
 (* end hide *)
 
@@ -894,9 +1242,7 @@ forall u1 t1 n1,
   degree_u_wrt_t (S n1) u1 ->
   degree_t_wrt_t n1 t1 ->
   degree_u_wrt_t n1 (open_u_wrt_t_rec n1 t1 u1).
-Proof.
-pose proof degree_u_wrt_t_open_u_wrt_t_rec_mutual as H; intuition eauto.
-Qed.
+Proof. Admitted.
 
 Hint Resolve degree_u_wrt_t_open_u_wrt_t_rec : lngen.
 
@@ -907,20 +1253,42 @@ forall t1 t2,
   degree_t_wrt_t 1 t1 ->
   degree_t_wrt_t 0 t2 ->
   degree_t_wrt_t 0 (open_t_wrt_t t1 t2).
-Proof.
-unfold open_t_wrt_t; default_simp.
-Qed.
+Proof. Admitted.
 
 Hint Resolve degree_t_wrt_t_open_t_wrt_t : lngen.
+
+Lemma degree_u_wrt_u_open_u_wrt_u :
+forall u1 u2,
+  degree_u_wrt_u 1 u1 ->
+  degree_u_wrt_u 0 u2 ->
+  degree_u_wrt_u 0 (open_u_wrt_u u1 u2).
+Proof. Admitted.
+
+Hint Resolve degree_u_wrt_u_open_u_wrt_u : lngen.
+
+Lemma degree_u_wrt_u_open_u_wrt_t :
+forall u1 t1 n1,
+  degree_u_wrt_u n1 u1 ->
+  degree_u_wrt_u n1 (open_u_wrt_t u1 t1).
+Proof. Admitted.
+
+Hint Resolve degree_u_wrt_u_open_u_wrt_t : lngen.
+
+Lemma degree_u_wrt_t_open_u_wrt_u :
+forall u1 u2 n1,
+  degree_u_wrt_t n1 u1 ->
+  degree_u_wrt_t n1 u2 ->
+  degree_u_wrt_t n1 (open_u_wrt_u u1 u2).
+Proof. Admitted.
+
+Hint Resolve degree_u_wrt_t_open_u_wrt_u : lngen.
 
 Lemma degree_u_wrt_t_open_u_wrt_t :
 forall u1 t1,
   degree_u_wrt_t 1 u1 ->
   degree_t_wrt_t 0 t1 ->
   degree_u_wrt_t 0 (open_u_wrt_t u1 t1).
-Proof.
-unfold open_u_wrt_t; default_simp.
-Qed.
+Proof. Admitted.
 
 Hint Resolve degree_u_wrt_t_open_u_wrt_t : lngen.
 
@@ -930,10 +1298,7 @@ Lemma degree_t_wrt_t_open_t_wrt_t_rec_inv_mutual :
 (forall t1 t2 n1,
   degree_t_wrt_t n1 (open_t_wrt_t_rec n1 t2 t1) ->
   degree_t_wrt_t (S n1) t1).
-Proof.
-apply_mutual_ind t_mutind;
-default_simp; eauto with lngen.
-Qed.
+Proof. Admitted.
 
 (* end hide *)
 
@@ -943,11 +1308,75 @@ Lemma degree_t_wrt_t_open_t_wrt_t_rec_inv :
 forall t1 t2 n1,
   degree_t_wrt_t n1 (open_t_wrt_t_rec n1 t2 t1) ->
   degree_t_wrt_t (S n1) t1.
-Proof.
-pose proof degree_t_wrt_t_open_t_wrt_t_rec_inv_mutual as H; intuition eauto.
-Qed.
+Proof. Admitted.
 
 Hint Immediate degree_t_wrt_t_open_t_wrt_t_rec_inv : lngen.
+
+(* end hide *)
+
+(* begin hide *)
+
+Lemma degree_u_wrt_u_open_u_wrt_u_rec_inv_mutual :
+(forall u1 u2 n1,
+  degree_u_wrt_u n1 (open_u_wrt_u_rec n1 u2 u1) ->
+  degree_u_wrt_u (S n1) u1).
+Proof. Admitted.
+
+(* end hide *)
+
+(* begin hide *)
+
+Lemma degree_u_wrt_u_open_u_wrt_u_rec_inv :
+forall u1 u2 n1,
+  degree_u_wrt_u n1 (open_u_wrt_u_rec n1 u2 u1) ->
+  degree_u_wrt_u (S n1) u1.
+Proof. Admitted.
+
+Hint Immediate degree_u_wrt_u_open_u_wrt_u_rec_inv : lngen.
+
+(* end hide *)
+
+(* begin hide *)
+
+Lemma degree_u_wrt_u_open_u_wrt_t_rec_inv_mutual :
+(forall u1 t1 n1 n2,
+  degree_u_wrt_u n1 (open_u_wrt_t_rec n2 t1 u1) ->
+  degree_u_wrt_u n1 u1).
+Proof. Admitted.
+
+(* end hide *)
+
+(* begin hide *)
+
+Lemma degree_u_wrt_u_open_u_wrt_t_rec_inv :
+forall u1 t1 n1 n2,
+  degree_u_wrt_u n1 (open_u_wrt_t_rec n2 t1 u1) ->
+  degree_u_wrt_u n1 u1.
+Proof. Admitted.
+
+Hint Immediate degree_u_wrt_u_open_u_wrt_t_rec_inv : lngen.
+
+(* end hide *)
+
+(* begin hide *)
+
+Lemma degree_u_wrt_t_open_u_wrt_u_rec_inv_mutual :
+(forall u1 u2 n1 n2,
+  degree_u_wrt_t n1 (open_u_wrt_u_rec n2 u2 u1) ->
+  degree_u_wrt_t n1 u1).
+Proof. Admitted.
+
+(* end hide *)
+
+(* begin hide *)
+
+Lemma degree_u_wrt_t_open_u_wrt_u_rec_inv :
+forall u1 u2 n1 n2,
+  degree_u_wrt_t n1 (open_u_wrt_u_rec n2 u2 u1) ->
+  degree_u_wrt_t n1 u1.
+Proof. Admitted.
+
+Hint Immediate degree_u_wrt_t_open_u_wrt_u_rec_inv : lngen.
 
 (* end hide *)
 
@@ -957,10 +1386,7 @@ Lemma degree_u_wrt_t_open_u_wrt_t_rec_inv_mutual :
 (forall u1 t1 n1,
   degree_u_wrt_t n1 (open_u_wrt_t_rec n1 t1 u1) ->
   degree_u_wrt_t (S n1) u1).
-Proof.
-apply_mutual_ind u_mutind;
-default_simp; eauto with lngen.
-Qed.
+Proof. Admitted.
 
 (* end hide *)
 
@@ -970,9 +1396,7 @@ Lemma degree_u_wrt_t_open_u_wrt_t_rec_inv :
 forall u1 t1 n1,
   degree_u_wrt_t n1 (open_u_wrt_t_rec n1 t1 u1) ->
   degree_u_wrt_t (S n1) u1.
-Proof.
-pose proof degree_u_wrt_t_open_u_wrt_t_rec_inv_mutual as H; intuition eauto.
-Qed.
+Proof. Admitted.
 
 Hint Immediate degree_u_wrt_t_open_u_wrt_t_rec_inv : lngen.
 
@@ -982,19 +1406,39 @@ Lemma degree_t_wrt_t_open_t_wrt_t_inv :
 forall t1 t2,
   degree_t_wrt_t 0 (open_t_wrt_t t1 t2) ->
   degree_t_wrt_t 1 t1.
-Proof.
-unfold open_t_wrt_t; eauto with lngen.
-Qed.
+Proof. Admitted.
 
 Hint Immediate degree_t_wrt_t_open_t_wrt_t_inv : lngen.
+
+Lemma degree_u_wrt_u_open_u_wrt_u_inv :
+forall u1 u2,
+  degree_u_wrt_u 0 (open_u_wrt_u u1 u2) ->
+  degree_u_wrt_u 1 u1.
+Proof. Admitted.
+
+Hint Immediate degree_u_wrt_u_open_u_wrt_u_inv : lngen.
+
+Lemma degree_u_wrt_u_open_u_wrt_t_inv :
+forall u1 t1 n1,
+  degree_u_wrt_u n1 (open_u_wrt_t u1 t1) ->
+  degree_u_wrt_u n1 u1.
+Proof. Admitted.
+
+Hint Immediate degree_u_wrt_u_open_u_wrt_t_inv : lngen.
+
+Lemma degree_u_wrt_t_open_u_wrt_u_inv :
+forall u1 u2 n1,
+  degree_u_wrt_t n1 (open_u_wrt_u u1 u2) ->
+  degree_u_wrt_t n1 u1.
+Proof. Admitted.
+
+Hint Immediate degree_u_wrt_t_open_u_wrt_u_inv : lngen.
 
 Lemma degree_u_wrt_t_open_u_wrt_t_inv :
 forall u1 t1,
   degree_u_wrt_t 0 (open_u_wrt_t u1 t1) ->
   degree_u_wrt_t 1 u1.
-Proof.
-unfold open_u_wrt_t; eauto with lngen.
-Qed.
+Proof. Admitted.
 
 Hint Immediate degree_u_wrt_t_open_u_wrt_t_inv : lngen.
 
@@ -1011,13 +1455,7 @@ Lemma close_t_wrt_t_rec_inj_mutual :
 (forall t1 t2 a1 n1,
   close_t_wrt_t_rec n1 a1 t1 = close_t_wrt_t_rec n1 a1 t2 ->
   t1 = t2).
-Proof.
-apply_mutual_ind t_mutind;
-intros; match goal with
-          | |- _ = ?term => destruct term
-        end;
-default_simp; eauto with lngen.
-Qed.
+Proof. Admitted.
 
 (* end hide *)
 
@@ -1027,11 +1465,31 @@ Lemma close_t_wrt_t_rec_inj :
 forall t1 t2 a1 n1,
   close_t_wrt_t_rec n1 a1 t1 = close_t_wrt_t_rec n1 a1 t2 ->
   t1 = t2.
-Proof.
-pose proof close_t_wrt_t_rec_inj_mutual as H; intuition eauto.
-Qed.
+Proof. Admitted.
 
 Hint Immediate close_t_wrt_t_rec_inj : lngen.
+
+(* end hide *)
+
+(* begin hide *)
+
+Lemma close_u_wrt_u_rec_inj_mutual :
+(forall u1 u2 x1 n1,
+  close_u_wrt_u_rec n1 x1 u1 = close_u_wrt_u_rec n1 x1 u2 ->
+  u1 = u2).
+Proof. Admitted.
+
+(* end hide *)
+
+(* begin hide *)
+
+Lemma close_u_wrt_u_rec_inj :
+forall u1 u2 x1 n1,
+  close_u_wrt_u_rec n1 x1 u1 = close_u_wrt_u_rec n1 x1 u2 ->
+  u1 = u2.
+Proof. Admitted.
+
+Hint Immediate close_u_wrt_u_rec_inj : lngen.
 
 (* end hide *)
 
@@ -1041,13 +1499,7 @@ Lemma close_u_wrt_t_rec_inj_mutual :
 (forall u1 u2 a1 n1,
   close_u_wrt_t_rec n1 a1 u1 = close_u_wrt_t_rec n1 a1 u2 ->
   u1 = u2).
-Proof.
-apply_mutual_ind u_mutind;
-intros; match goal with
-          | |- _ = ?term => destruct term
-        end;
-default_simp; eauto with lngen.
-Qed.
+Proof. Admitted.
 
 (* end hide *)
 
@@ -1057,9 +1509,7 @@ Lemma close_u_wrt_t_rec_inj :
 forall u1 u2 a1 n1,
   close_u_wrt_t_rec n1 a1 u1 = close_u_wrt_t_rec n1 a1 u2 ->
   u1 = u2.
-Proof.
-pose proof close_u_wrt_t_rec_inj_mutual as H; intuition eauto.
-Qed.
+Proof. Admitted.
 
 Hint Immediate close_u_wrt_t_rec_inj : lngen.
 
@@ -1069,19 +1519,23 @@ Lemma close_t_wrt_t_inj :
 forall t1 t2 a1,
   close_t_wrt_t a1 t1 = close_t_wrt_t a1 t2 ->
   t1 = t2.
-Proof.
-unfold close_t_wrt_t; eauto with lngen.
-Qed.
+Proof. Admitted.
 
 Hint Immediate close_t_wrt_t_inj : lngen.
+
+Lemma close_u_wrt_u_inj :
+forall u1 u2 x1,
+  close_u_wrt_u x1 u1 = close_u_wrt_u x1 u2 ->
+  u1 = u2.
+Proof. Admitted.
+
+Hint Immediate close_u_wrt_u_inj : lngen.
 
 Lemma close_u_wrt_t_inj :
 forall u1 u2 a1,
   close_u_wrt_t a1 u1 = close_u_wrt_t a1 u2 ->
   u1 = u2.
-Proof.
-unfold close_u_wrt_t; eauto with lngen.
-Qed.
+Proof. Admitted.
 
 Hint Immediate close_u_wrt_t_inj : lngen.
 
@@ -1091,10 +1545,7 @@ Lemma close_t_wrt_t_rec_open_t_wrt_t_rec_mutual :
 (forall t1 a1 n1,
   a1 `notin` tt_fv_t t1 ->
   close_t_wrt_t_rec n1 a1 (open_t_wrt_t_rec n1 (t_var_f a1) t1) = t1).
-Proof.
-apply_mutual_ind t_mutind;
-default_simp.
-Qed.
+Proof. Admitted.
 
 (* end hide *)
 
@@ -1104,12 +1555,33 @@ Lemma close_t_wrt_t_rec_open_t_wrt_t_rec :
 forall t1 a1 n1,
   a1 `notin` tt_fv_t t1 ->
   close_t_wrt_t_rec n1 a1 (open_t_wrt_t_rec n1 (t_var_f a1) t1) = t1.
-Proof.
-pose proof close_t_wrt_t_rec_open_t_wrt_t_rec_mutual as H; intuition eauto.
-Qed.
+Proof. Admitted.
 
 Hint Resolve close_t_wrt_t_rec_open_t_wrt_t_rec : lngen.
 Hint Rewrite close_t_wrt_t_rec_open_t_wrt_t_rec using solve [auto] : lngen.
+
+(* end hide *)
+
+(* begin hide *)
+
+Lemma close_u_wrt_u_rec_open_u_wrt_u_rec_mutual :
+(forall u1 x1 n1,
+  x1 `notin` e_fv_u u1 ->
+  close_u_wrt_u_rec n1 x1 (open_u_wrt_u_rec n1 (u_var_f x1) u1) = u1).
+Proof. Admitted.
+
+(* end hide *)
+
+(* begin hide *)
+
+Lemma close_u_wrt_u_rec_open_u_wrt_u_rec :
+forall u1 x1 n1,
+  x1 `notin` e_fv_u u1 ->
+  close_u_wrt_u_rec n1 x1 (open_u_wrt_u_rec n1 (u_var_f x1) u1) = u1.
+Proof. Admitted.
+
+Hint Resolve close_u_wrt_u_rec_open_u_wrt_u_rec : lngen.
+Hint Rewrite close_u_wrt_u_rec_open_u_wrt_u_rec using solve [auto] : lngen.
 
 (* end hide *)
 
@@ -1119,10 +1591,7 @@ Lemma close_u_wrt_t_rec_open_u_wrt_t_rec_mutual :
 (forall u1 a1 n1,
   a1 `notin` tt_fv_u u1 ->
   close_u_wrt_t_rec n1 a1 (open_u_wrt_t_rec n1 (t_var_f a1) u1) = u1).
-Proof.
-apply_mutual_ind u_mutind;
-default_simp.
-Qed.
+Proof. Admitted.
 
 (* end hide *)
 
@@ -1132,9 +1601,7 @@ Lemma close_u_wrt_t_rec_open_u_wrt_t_rec :
 forall u1 a1 n1,
   a1 `notin` tt_fv_u u1 ->
   close_u_wrt_t_rec n1 a1 (open_u_wrt_t_rec n1 (t_var_f a1) u1) = u1.
-Proof.
-pose proof close_u_wrt_t_rec_open_u_wrt_t_rec_mutual as H; intuition eauto.
-Qed.
+Proof. Admitted.
 
 Hint Resolve close_u_wrt_t_rec_open_u_wrt_t_rec : lngen.
 Hint Rewrite close_u_wrt_t_rec_open_u_wrt_t_rec using solve [auto] : lngen.
@@ -1145,20 +1612,25 @@ Lemma close_t_wrt_t_open_t_wrt_t :
 forall t1 a1,
   a1 `notin` tt_fv_t t1 ->
   close_t_wrt_t a1 (open_t_wrt_t t1 (t_var_f a1)) = t1.
-Proof.
-unfold close_t_wrt_t; unfold open_t_wrt_t; default_simp.
-Qed.
+Proof. Admitted.
 
 Hint Resolve close_t_wrt_t_open_t_wrt_t : lngen.
 Hint Rewrite close_t_wrt_t_open_t_wrt_t using solve [auto] : lngen.
+
+Lemma close_u_wrt_u_open_u_wrt_u :
+forall u1 x1,
+  x1 `notin` e_fv_u u1 ->
+  close_u_wrt_u x1 (open_u_wrt_u u1 (u_var_f x1)) = u1.
+Proof. Admitted.
+
+Hint Resolve close_u_wrt_u_open_u_wrt_u : lngen.
+Hint Rewrite close_u_wrt_u_open_u_wrt_u using solve [auto] : lngen.
 
 Lemma close_u_wrt_t_open_u_wrt_t :
 forall u1 a1,
   a1 `notin` tt_fv_u u1 ->
   close_u_wrt_t a1 (open_u_wrt_t u1 (t_var_f a1)) = u1.
-Proof.
-unfold close_u_wrt_t; unfold open_u_wrt_t; default_simp.
-Qed.
+Proof. Admitted.
 
 Hint Resolve close_u_wrt_t_open_u_wrt_t : lngen.
 Hint Rewrite close_u_wrt_t_open_u_wrt_t using solve [auto] : lngen.
@@ -1168,10 +1640,7 @@ Hint Rewrite close_u_wrt_t_open_u_wrt_t using solve [auto] : lngen.
 Lemma open_t_wrt_t_rec_close_t_wrt_t_rec_mutual :
 (forall t1 a1 n1,
   open_t_wrt_t_rec n1 (t_var_f a1) (close_t_wrt_t_rec n1 a1 t1) = t1).
-Proof.
-apply_mutual_ind t_mutind;
-default_simp.
-Qed.
+Proof. Admitted.
 
 (* end hide *)
 
@@ -1180,9 +1649,7 @@ Qed.
 Lemma open_t_wrt_t_rec_close_t_wrt_t_rec :
 forall t1 a1 n1,
   open_t_wrt_t_rec n1 (t_var_f a1) (close_t_wrt_t_rec n1 a1 t1) = t1.
-Proof.
-pose proof open_t_wrt_t_rec_close_t_wrt_t_rec_mutual as H; intuition eauto.
-Qed.
+Proof. Admitted.
 
 Hint Resolve open_t_wrt_t_rec_close_t_wrt_t_rec : lngen.
 Hint Rewrite open_t_wrt_t_rec_close_t_wrt_t_rec using solve [auto] : lngen.
@@ -1191,13 +1658,31 @@ Hint Rewrite open_t_wrt_t_rec_close_t_wrt_t_rec using solve [auto] : lngen.
 
 (* begin hide *)
 
+Lemma open_u_wrt_u_rec_close_u_wrt_u_rec_mutual :
+(forall u1 x1 n1,
+  open_u_wrt_u_rec n1 (u_var_f x1) (close_u_wrt_u_rec n1 x1 u1) = u1).
+Proof. Admitted.
+
+(* end hide *)
+
+(* begin hide *)
+
+Lemma open_u_wrt_u_rec_close_u_wrt_u_rec :
+forall u1 x1 n1,
+  open_u_wrt_u_rec n1 (u_var_f x1) (close_u_wrt_u_rec n1 x1 u1) = u1.
+Proof. Admitted.
+
+Hint Resolve open_u_wrt_u_rec_close_u_wrt_u_rec : lngen.
+Hint Rewrite open_u_wrt_u_rec_close_u_wrt_u_rec using solve [auto] : lngen.
+
+(* end hide *)
+
+(* begin hide *)
+
 Lemma open_u_wrt_t_rec_close_u_wrt_t_rec_mutual :
 (forall u1 a1 n1,
   open_u_wrt_t_rec n1 (t_var_f a1) (close_u_wrt_t_rec n1 a1 u1) = u1).
-Proof.
-apply_mutual_ind u_mutind;
-default_simp.
-Qed.
+Proof. Admitted.
 
 (* end hide *)
 
@@ -1206,9 +1691,7 @@ Qed.
 Lemma open_u_wrt_t_rec_close_u_wrt_t_rec :
 forall u1 a1 n1,
   open_u_wrt_t_rec n1 (t_var_f a1) (close_u_wrt_t_rec n1 a1 u1) = u1.
-Proof.
-pose proof open_u_wrt_t_rec_close_u_wrt_t_rec_mutual as H; intuition eauto.
-Qed.
+Proof. Admitted.
 
 Hint Resolve open_u_wrt_t_rec_close_u_wrt_t_rec : lngen.
 Hint Rewrite open_u_wrt_t_rec_close_u_wrt_t_rec using solve [auto] : lngen.
@@ -1218,19 +1701,23 @@ Hint Rewrite open_u_wrt_t_rec_close_u_wrt_t_rec using solve [auto] : lngen.
 Lemma open_t_wrt_t_close_t_wrt_t :
 forall t1 a1,
   open_t_wrt_t (close_t_wrt_t a1 t1) (t_var_f a1) = t1.
-Proof.
-unfold close_t_wrt_t; unfold open_t_wrt_t; default_simp.
-Qed.
+Proof. Admitted.
 
 Hint Resolve open_t_wrt_t_close_t_wrt_t : lngen.
 Hint Rewrite open_t_wrt_t_close_t_wrt_t using solve [auto] : lngen.
 
+Lemma open_u_wrt_u_close_u_wrt_u :
+forall u1 x1,
+  open_u_wrt_u (close_u_wrt_u x1 u1) (u_var_f x1) = u1.
+Proof. Admitted.
+
+Hint Resolve open_u_wrt_u_close_u_wrt_u : lngen.
+Hint Rewrite open_u_wrt_u_close_u_wrt_u using solve [auto] : lngen.
+
 Lemma open_u_wrt_t_close_u_wrt_t :
 forall u1 a1,
   open_u_wrt_t (close_u_wrt_t a1 u1) (t_var_f a1) = u1.
-Proof.
-unfold close_u_wrt_t; unfold open_u_wrt_t; default_simp.
-Qed.
+Proof. Admitted.
 
 Hint Resolve open_u_wrt_t_close_u_wrt_t : lngen.
 Hint Rewrite open_u_wrt_t_close_u_wrt_t using solve [auto] : lngen.
@@ -1243,13 +1730,7 @@ Lemma open_t_wrt_t_rec_inj_mutual :
   a1 `notin` tt_fv_t t1 ->
   open_t_wrt_t_rec n1 (t_var_f a1) t2 = open_t_wrt_t_rec n1 (t_var_f a1) t1 ->
   t2 = t1).
-Proof.
-apply_mutual_ind t_mutind;
-intros; match goal with
-          | |- _ = ?term => destruct term
-        end;
-default_simp; eauto with lngen.
-Qed.
+Proof. Admitted.
 
 (* end hide *)
 
@@ -1261,11 +1742,35 @@ forall t2 t1 a1 n1,
   a1 `notin` tt_fv_t t1 ->
   open_t_wrt_t_rec n1 (t_var_f a1) t2 = open_t_wrt_t_rec n1 (t_var_f a1) t1 ->
   t2 = t1.
-Proof.
-pose proof open_t_wrt_t_rec_inj_mutual as H; intuition eauto.
-Qed.
+Proof. Admitted.
 
 Hint Immediate open_t_wrt_t_rec_inj : lngen.
+
+(* end hide *)
+
+(* begin hide *)
+
+Lemma open_u_wrt_u_rec_inj_mutual :
+(forall u2 u1 x1 n1,
+  x1 `notin` e_fv_u u2 ->
+  x1 `notin` e_fv_u u1 ->
+  open_u_wrt_u_rec n1 (u_var_f x1) u2 = open_u_wrt_u_rec n1 (u_var_f x1) u1 ->
+  u2 = u1).
+Proof. Admitted.
+
+(* end hide *)
+
+(* begin hide *)
+
+Lemma open_u_wrt_u_rec_inj :
+forall u2 u1 x1 n1,
+  x1 `notin` e_fv_u u2 ->
+  x1 `notin` e_fv_u u1 ->
+  open_u_wrt_u_rec n1 (u_var_f x1) u2 = open_u_wrt_u_rec n1 (u_var_f x1) u1 ->
+  u2 = u1.
+Proof. Admitted.
+
+Hint Immediate open_u_wrt_u_rec_inj : lngen.
 
 (* end hide *)
 
@@ -1277,13 +1782,7 @@ Lemma open_u_wrt_t_rec_inj_mutual :
   a1 `notin` tt_fv_u u1 ->
   open_u_wrt_t_rec n1 (t_var_f a1) u2 = open_u_wrt_t_rec n1 (t_var_f a1) u1 ->
   u2 = u1).
-Proof.
-apply_mutual_ind u_mutind;
-intros; match goal with
-          | |- _ = ?term => destruct term
-        end;
-default_simp; eauto with lngen.
-Qed.
+Proof. Admitted.
 
 (* end hide *)
 
@@ -1295,9 +1794,7 @@ forall u2 u1 a1 n1,
   a1 `notin` tt_fv_u u1 ->
   open_u_wrt_t_rec n1 (t_var_f a1) u2 = open_u_wrt_t_rec n1 (t_var_f a1) u1 ->
   u2 = u1.
-Proof.
-pose proof open_u_wrt_t_rec_inj_mutual as H; intuition eauto.
-Qed.
+Proof. Admitted.
 
 Hint Immediate open_u_wrt_t_rec_inj : lngen.
 
@@ -1309,11 +1806,19 @@ forall t2 t1 a1,
   a1 `notin` tt_fv_t t1 ->
   open_t_wrt_t t2 (t_var_f a1) = open_t_wrt_t t1 (t_var_f a1) ->
   t2 = t1.
-Proof.
-unfold open_t_wrt_t; eauto with lngen.
-Qed.
+Proof. Admitted.
 
 Hint Immediate open_t_wrt_t_inj : lngen.
+
+Lemma open_u_wrt_u_inj :
+forall u2 u1 x1,
+  x1 `notin` e_fv_u u2 ->
+  x1 `notin` e_fv_u u1 ->
+  open_u_wrt_u u2 (u_var_f x1) = open_u_wrt_u u1 (u_var_f x1) ->
+  u2 = u1.
+Proof. Admitted.
+
+Hint Immediate open_u_wrt_u_inj : lngen.
 
 Lemma open_u_wrt_t_inj :
 forall u2 u1 a1,
@@ -1321,9 +1826,7 @@ forall u2 u1 a1,
   a1 `notin` tt_fv_u u1 ->
   open_u_wrt_t u2 (t_var_f a1) = open_u_wrt_t u1 (t_var_f a1) ->
   u2 = u1.
-Proof.
-unfold open_u_wrt_t; eauto with lngen.
-Qed.
+Proof. Admitted.
 
 Hint Immediate open_u_wrt_t_inj : lngen.
 
@@ -1340,15 +1843,7 @@ Lemma degree_t_wrt_t_of_lc_t_mutual :
 (forall t1,
   lc_t t1 ->
   degree_t_wrt_t 0 t1).
-Proof.
-apply_mutual_ind lc_t_mutind;
-intros;
-let a1 := fresh "a1" in pick_fresh a1;
-repeat (match goal with
-          | H1 : _, H2 : _ |- _ => specialize H1 with H2
-        end);
-default_simp; eauto with lngen.
-Qed.
+Proof. Admitted.
 
 (* end hide *)
 
@@ -1356,11 +1851,27 @@ Lemma degree_t_wrt_t_of_lc_t :
 forall t1,
   lc_t t1 ->
   degree_t_wrt_t 0 t1.
-Proof.
-pose proof degree_t_wrt_t_of_lc_t_mutual as H; intuition eauto.
-Qed.
+Proof. Admitted.
 
 Hint Resolve degree_t_wrt_t_of_lc_t : lngen.
+
+(* begin hide *)
+
+Lemma degree_u_wrt_u_of_lc_u_mutual :
+(forall u1,
+  lc_u u1 ->
+  degree_u_wrt_u 0 u1).
+Proof. Admitted.
+
+(* end hide *)
+
+Lemma degree_u_wrt_u_of_lc_u :
+forall u1,
+  lc_u u1 ->
+  degree_u_wrt_u 0 u1.
+Proof. Admitted.
+
+Hint Resolve degree_u_wrt_u_of_lc_u : lngen.
 
 (* begin hide *)
 
@@ -1368,15 +1879,7 @@ Lemma degree_u_wrt_t_of_lc_u_mutual :
 (forall u1,
   lc_u u1 ->
   degree_u_wrt_t 0 u1).
-Proof.
-apply_mutual_ind lc_u_mutind;
-intros;
-let a1 := fresh "a1" in pick_fresh a1;
-repeat (match goal with
-          | H1 : _, H2 : _ |- _ => specialize H1 with H2
-        end);
-default_simp; eauto with lngen.
-Qed.
+Proof. Admitted.
 
 (* end hide *)
 
@@ -1384,9 +1887,7 @@ Lemma degree_u_wrt_t_of_lc_u :
 forall u1,
   lc_u u1 ->
   degree_u_wrt_t 0 u1.
-Proof.
-pose proof degree_u_wrt_t_of_lc_u_mutual as H; intuition eauto.
-Qed.
+Proof. Admitted.
 
 Hint Resolve degree_u_wrt_t_of_lc_u : lngen.
 
@@ -1398,22 +1899,7 @@ forall i1,
   size_t t1 = i1 ->
   degree_t_wrt_t 0 t1 ->
   lc_t t1).
-Proof.
-intros i1; pattern i1; apply lt_wf_rec;
-clear i1; intros i1 H1;
-apply_mutual_ind t_mutind;
-default_simp;
-(* non-trivial cases *)
-constructor; default_simp; eapply_first_hyp;
-(* instantiate the size *)
-match goal with
-  | |- _ = _ => reflexivity
-  | _ => idtac
-end;
-instantiate;
-(* everything should be easy now *)
-default_simp.
-Qed.
+Proof. Admitted.
 
 (* end hide *)
 
@@ -1421,11 +1907,7 @@ Lemma lc_t_of_degree :
 forall t1,
   degree_t_wrt_t 0 t1 ->
   lc_t t1.
-Proof.
-intros t1; intros;
-pose proof (lc_t_of_degree_size_mutual (size_t t1));
-intuition eauto.
-Qed.
+Proof. Admitted.
 
 Hint Resolve lc_t_of_degree : lngen.
 
@@ -1435,36 +1917,19 @@ Lemma lc_u_of_degree_size_mutual :
 forall i1,
 (forall u1,
   size_u u1 = i1 ->
+  degree_u_wrt_u 0 u1 ->
   degree_u_wrt_t 0 u1 ->
   lc_u u1).
-Proof.
-intros i1; pattern i1; apply lt_wf_rec;
-clear i1; intros i1 H1;
-apply_mutual_ind u_mutind;
-default_simp;
-(* non-trivial cases *)
-constructor; default_simp; eapply_first_hyp;
-(* instantiate the size *)
-match goal with
-  | |- _ = _ => reflexivity
-  | _ => idtac
-end;
-instantiate;
-(* everything should be easy now *)
-default_simp.
-Qed.
+Proof. Admitted.
 
 (* end hide *)
 
 Lemma lc_u_of_degree :
 forall u1,
+  degree_u_wrt_u 0 u1 ->
   degree_u_wrt_t 0 u1 ->
   lc_u u1.
-Proof.
-intros u1; intros;
-pose proof (lc_u_of_degree_size_mutual (size_u u1));
-intuition eauto.
-Qed.
+Proof. Admitted.
 
 Hint Resolve lc_u_of_degree : lngen.
 
@@ -1483,29 +1948,51 @@ Ltac p_lc_exists_tac :=
 Ltac u_lc_exists_tac :=
   repeat (match goal with
             | H : _ |- _ =>
-              let J1 := fresh in pose proof H as J1; apply degree_u_wrt_t_of_lc_u in J1; clear H
+              let J1 := fresh in pose proof H as J1; apply degree_u_wrt_u_of_lc_u in J1;
+              let J2 := fresh in pose proof H as J2; apply degree_u_wrt_t_of_lc_u in J2; clear H
           end).
 
 Lemma lc_t_all_exists :
 forall a1 t1,
   lc_t (open_t_wrt_t t1 (t_var_f a1)) ->
   lc_t (t_all t1).
-Proof.
-intros; t_lc_exists_tac; eauto with lngen.
-Qed.
+Proof. Admitted.
+
+Lemma lc_u_fix_exists :
+forall x1 t1 t2 e1,
+  lc_t t1 ->
+  lc_t t2 ->
+  lc_u (open_u_wrt_u e1 (u_var_f x1)) ->
+  lc_u (u_fix t1 t2 e1).
+Proof. Admitted.
+
+Lemma lc_u_lam_exists :
+forall x1 t1 e1,
+  lc_t t1 ->
+  lc_u (open_u_wrt_u e1 (u_var_f x1)) ->
+  lc_u (u_lam t1 e1).
+Proof. Admitted.
 
 Lemma lc_u_tlam_exists :
 forall a1 e1,
   lc_u (open_u_wrt_t e1 (t_var_f a1)) ->
   lc_u (u_tlam e1).
-Proof.
-intros; u_lc_exists_tac; eauto with lngen.
-Qed.
+Proof. Admitted.
 
 Hint Extern 1 (lc_t (t_all _)) =>
   let a1 := fresh in
   pick_fresh a1;
   apply (lc_t_all_exists a1).
+
+Hint Extern 1 (lc_u (u_fix _ _ _)) =>
+  let x1 := fresh in
+  pick_fresh x1;
+  apply (lc_u_fix_exists x1).
+
+Hint Extern 1 (lc_u (u_lam _ _)) =>
+  let x1 := fresh in
+  pick_fresh x1;
+  apply (lc_u_lam_exists x1).
 
 Hint Extern 1 (lc_u (u_tlam _)) =>
   let a1 := fresh in
@@ -1517,32 +2004,25 @@ forall t1 t2,
   body_t_wrt_t t1 ->
   lc_t t2 ->
   lc_t (open_t_wrt_t t1 t2).
-Proof.
-unfold body_t_wrt_t;
-default_simp;
-let a1 := fresh "x" in
-pick_fresh a1;
-specialize_all a1;
-t_lc_exists_tac;
-eauto with lngen.
-Qed.
+Proof. Admitted.
 
 Hint Resolve lc_body_t_wrt_t : lngen.
+
+Lemma lc_body_u_wrt_u :
+forall u1 u2,
+  body_u_wrt_u u1 ->
+  lc_u u2 ->
+  lc_u (open_u_wrt_u u1 u2).
+Proof. Admitted.
+
+Hint Resolve lc_body_u_wrt_u : lngen.
 
 Lemma lc_body_u_wrt_t :
 forall u1 t1,
   body_u_wrt_t u1 ->
   lc_t t1 ->
   lc_u (open_u_wrt_t u1 t1).
-Proof.
-unfold body_u_wrt_t;
-default_simp;
-let a1 := fresh "x" in
-pick_fresh a1;
-specialize_all a1;
-u_lc_exists_tac;
-eauto with lngen.
-Qed.
+Proof. Admitted.
 
 Hint Resolve lc_body_u_wrt_t : lngen.
 
@@ -1550,19 +2030,31 @@ Lemma lc_body_t_all_1 :
 forall t1,
   lc_t (t_all t1) ->
   body_t_wrt_t t1.
-Proof.
-default_simp.
-Qed.
+Proof. Admitted.
 
 Hint Resolve lc_body_t_all_1 : lngen.
+
+Lemma lc_body_u_fix_3 :
+forall t1 t2 e1,
+  lc_u (u_fix t1 t2 e1) ->
+  body_u_wrt_u e1.
+Proof. Admitted.
+
+Hint Resolve lc_body_u_fix_3 : lngen.
+
+Lemma lc_body_u_lam_2 :
+forall t1 e1,
+  lc_u (u_lam t1 e1) ->
+  body_u_wrt_u e1.
+Proof. Admitted.
+
+Hint Resolve lc_body_u_lam_2 : lngen.
 
 Lemma lc_body_u_tlam_1 :
 forall e1,
   lc_u (u_tlam e1) ->
   body_u_wrt_t e1.
-Proof.
-default_simp.
-Qed.
+Proof. Admitted.
 
 Hint Resolve lc_body_u_tlam_1 : lngen.
 
@@ -1570,21 +2062,13 @@ Hint Resolve lc_body_u_tlam_1 : lngen.
 
 Lemma lc_t_unique_mutual :
 (forall t1 (proof2 proof3 : lc_t t1), proof2 = proof3).
-Proof.
-apply_mutual_ind lc_t_mutind;
-intros;
-let proof1 := fresh "proof1" in
-rename_last_into proof1; dependent destruction proof1;
-f_equal; default_simp; auto using @functional_extensionality_dep with lngen.
-Qed.
+Proof. Admitted.
 
 (* end hide *)
 
 Lemma lc_t_unique :
 forall t1 (proof2 proof3 : lc_t t1), proof2 = proof3.
-Proof.
-pose proof lc_t_unique_mutual as H; intuition eauto.
-Qed.
+Proof. Admitted.
 
 Hint Resolve lc_t_unique : lngen.
 
@@ -1592,21 +2076,13 @@ Hint Resolve lc_t_unique : lngen.
 
 Lemma lc_u_unique_mutual :
 (forall u1 (proof2 proof3 : lc_u u1), proof2 = proof3).
-Proof.
-apply_mutual_ind lc_u_mutind;
-intros;
-let proof1 := fresh "proof1" in
-rename_last_into proof1; dependent destruction proof1;
-f_equal; default_simp; auto using @functional_extensionality_dep with lngen.
-Qed.
+Proof. Admitted.
 
 (* end hide *)
 
 Lemma lc_u_unique :
 forall u1 (proof2 proof3 : lc_u u1), proof2 = proof3.
-Proof.
-pose proof lc_u_unique_mutual as H; intuition eauto.
-Qed.
+Proof. Admitted.
 
 Hint Resolve lc_u_unique : lngen.
 
@@ -1614,18 +2090,13 @@ Hint Resolve lc_u_unique : lngen.
 
 Lemma lc_t_of_lc_set_t_mutual :
 (forall t1, lc_set_t t1 -> lc_t t1).
-Proof.
-apply_mutual_ind lc_set_t_mutind;
-default_simp.
-Qed.
+Proof. Admitted.
 
 (* end hide *)
 
 Lemma lc_t_of_lc_set_t :
 forall t1, lc_set_t t1 -> lc_t t1.
-Proof.
-pose proof lc_t_of_lc_set_t_mutual as H; intuition eauto.
-Qed.
+Proof. Admitted.
 
 Hint Resolve lc_t_of_lc_set_t : lngen.
 
@@ -1633,18 +2104,13 @@ Hint Resolve lc_t_of_lc_set_t : lngen.
 
 Lemma lc_u_of_lc_set_u_mutual :
 (forall u1, lc_set_u u1 -> lc_u u1).
-Proof.
-apply_mutual_ind lc_set_u_mutind;
-default_simp.
-Qed.
+Proof. Admitted.
 
 (* end hide *)
 
 Lemma lc_u_of_lc_set_u :
 forall u1, lc_set_u u1 -> lc_u u1.
-Proof.
-pose proof lc_u_of_lc_set_u_mutual as H; intuition eauto.
-Qed.
+Proof. Admitted.
 
 Hint Resolve lc_u_of_lc_set_u : lngen.
 
@@ -1656,25 +2122,7 @@ forall i1,
   size_t t1 = i1 ->
   lc_t t1 ->
   lc_set_t t1).
-Proof.
-intros i1; pattern i1; apply lt_wf_rec;
-clear i1; intros i1 H1;
-apply_mutual_ind t_mutrec;
-default_simp;
-try solve [assert False by default_simp; tauto];
-(* non-trivial cases *)
-constructor; default_simp;
-try first [apply lc_set_t_of_lc_t];
-default_simp; eapply_first_hyp;
-(* instantiate the size *)
-match goal with
-  | |- _ = _ => reflexivity
-  | _ => idtac
-end;
-instantiate;
-(* everything should be easy now *)
-default_simp.
-Qed.
+Proof. Admitted.
 
 (* end hide *)
 
@@ -1682,11 +2130,7 @@ Lemma lc_set_t_of_lc_t :
 forall t1,
   lc_t t1 ->
   lc_set_t t1.
-Proof.
-intros t1; intros;
-pose proof (lc_set_t_of_lc_t_size_mutual (size_t t1));
-intuition eauto.
-Qed.
+Proof. Admitted.
 
 Hint Resolve lc_set_t_of_lc_t : lngen.
 
@@ -1698,27 +2142,7 @@ forall i1,
   size_u u1 = i1 ->
   lc_u u1 ->
   lc_set_u u1).
-Proof.
-intros i1; pattern i1; apply lt_wf_rec;
-clear i1; intros i1 H1;
-apply_mutual_ind u_mutrec;
-default_simp;
-try solve [assert False by default_simp; tauto];
-(* non-trivial cases *)
-constructor; default_simp;
-try first [apply lc_set_u_of_lc_u
- | apply lc_set_p_of_lc_p
- | apply lc_set_t_of_lc_t];
-default_simp; eapply_first_hyp;
-(* instantiate the size *)
-match goal with
-  | |- _ = _ => reflexivity
-  | _ => idtac
-end;
-instantiate;
-(* everything should be easy now *)
-default_simp.
-Qed.
+Proof. Admitted.
 
 (* end hide *)
 
@@ -1726,11 +2150,7 @@ Lemma lc_set_u_of_lc_u :
 forall u1,
   lc_u u1 ->
   lc_set_u u1.
-Proof.
-intros u1; intros;
-pose proof (lc_set_u_of_lc_u_size_mutual (size_u u1));
-intuition eauto.
-Qed.
+Proof. Admitted.
 
 Hint Resolve lc_set_u_of_lc_u : lngen.
 
@@ -1748,10 +2168,7 @@ Lemma close_t_wrt_t_rec_degree_t_wrt_t_mutual :
   degree_t_wrt_t n1 t1 ->
   a1 `notin` tt_fv_t t1 ->
   close_t_wrt_t_rec n1 a1 t1 = t1).
-Proof.
-apply_mutual_ind t_mutind;
-default_simp.
-Qed.
+Proof. Admitted.
 
 (* end hide *)
 
@@ -1762,12 +2179,35 @@ forall t1 a1 n1,
   degree_t_wrt_t n1 t1 ->
   a1 `notin` tt_fv_t t1 ->
   close_t_wrt_t_rec n1 a1 t1 = t1.
-Proof.
-pose proof close_t_wrt_t_rec_degree_t_wrt_t_mutual as H; intuition eauto.
-Qed.
+Proof. Admitted.
 
 Hint Resolve close_t_wrt_t_rec_degree_t_wrt_t : lngen.
 Hint Rewrite close_t_wrt_t_rec_degree_t_wrt_t using solve [auto] : lngen.
+
+(* end hide *)
+
+(* begin hide *)
+
+Lemma close_u_wrt_u_rec_degree_u_wrt_u_mutual :
+(forall u1 x1 n1,
+  degree_u_wrt_u n1 u1 ->
+  x1 `notin` e_fv_u u1 ->
+  close_u_wrt_u_rec n1 x1 u1 = u1).
+Proof. Admitted.
+
+(* end hide *)
+
+(* begin hide *)
+
+Lemma close_u_wrt_u_rec_degree_u_wrt_u :
+forall u1 x1 n1,
+  degree_u_wrt_u n1 u1 ->
+  x1 `notin` e_fv_u u1 ->
+  close_u_wrt_u_rec n1 x1 u1 = u1.
+Proof. Admitted.
+
+Hint Resolve close_u_wrt_u_rec_degree_u_wrt_u : lngen.
+Hint Rewrite close_u_wrt_u_rec_degree_u_wrt_u using solve [auto] : lngen.
 
 (* end hide *)
 
@@ -1778,10 +2218,7 @@ Lemma close_u_wrt_t_rec_degree_u_wrt_t_mutual :
   degree_u_wrt_t n1 u1 ->
   a1 `notin` tt_fv_u u1 ->
   close_u_wrt_t_rec n1 a1 u1 = u1).
-Proof.
-apply_mutual_ind u_mutind;
-default_simp.
-Qed.
+Proof. Admitted.
 
 (* end hide *)
 
@@ -1792,9 +2229,7 @@ forall u1 a1 n1,
   degree_u_wrt_t n1 u1 ->
   a1 `notin` tt_fv_u u1 ->
   close_u_wrt_t_rec n1 a1 u1 = u1.
-Proof.
-pose proof close_u_wrt_t_rec_degree_u_wrt_t_mutual as H; intuition eauto.
-Qed.
+Proof. Admitted.
 
 Hint Resolve close_u_wrt_t_rec_degree_u_wrt_t : lngen.
 Hint Rewrite close_u_wrt_t_rec_degree_u_wrt_t using solve [auto] : lngen.
@@ -1806,21 +2241,27 @@ forall t1 a1,
   lc_t t1 ->
   a1 `notin` tt_fv_t t1 ->
   close_t_wrt_t a1 t1 = t1.
-Proof.
-unfold close_t_wrt_t; default_simp.
-Qed.
+Proof. Admitted.
 
 Hint Resolve close_t_wrt_t_lc_t : lngen.
 Hint Rewrite close_t_wrt_t_lc_t using solve [auto] : lngen.
+
+Lemma close_u_wrt_u_lc_u :
+forall u1 x1,
+  lc_u u1 ->
+  x1 `notin` e_fv_u u1 ->
+  close_u_wrt_u x1 u1 = u1.
+Proof. Admitted.
+
+Hint Resolve close_u_wrt_u_lc_u : lngen.
+Hint Rewrite close_u_wrt_u_lc_u using solve [auto] : lngen.
 
 Lemma close_u_wrt_t_lc_u :
 forall u1 a1,
   lc_u u1 ->
   a1 `notin` tt_fv_u u1 ->
   close_u_wrt_t a1 u1 = u1.
-Proof.
-unfold close_u_wrt_t; default_simp.
-Qed.
+Proof. Admitted.
 
 Hint Resolve close_u_wrt_t_lc_u : lngen.
 Hint Rewrite close_u_wrt_t_lc_u using solve [auto] : lngen.
@@ -1831,10 +2272,7 @@ Lemma open_t_wrt_t_rec_degree_t_wrt_t_mutual :
 (forall t2 t1 n1,
   degree_t_wrt_t n1 t2 ->
   open_t_wrt_t_rec n1 t1 t2 = t2).
-Proof.
-apply_mutual_ind t_mutind;
-default_simp.
-Qed.
+Proof. Admitted.
 
 (* end hide *)
 
@@ -1844,12 +2282,33 @@ Lemma open_t_wrt_t_rec_degree_t_wrt_t :
 forall t2 t1 n1,
   degree_t_wrt_t n1 t2 ->
   open_t_wrt_t_rec n1 t1 t2 = t2.
-Proof.
-pose proof open_t_wrt_t_rec_degree_t_wrt_t_mutual as H; intuition eauto.
-Qed.
+Proof. Admitted.
 
 Hint Resolve open_t_wrt_t_rec_degree_t_wrt_t : lngen.
 Hint Rewrite open_t_wrt_t_rec_degree_t_wrt_t using solve [auto] : lngen.
+
+(* end hide *)
+
+(* begin hide *)
+
+Lemma open_u_wrt_u_rec_degree_u_wrt_u_mutual :
+(forall u2 u1 n1,
+  degree_u_wrt_u n1 u2 ->
+  open_u_wrt_u_rec n1 u1 u2 = u2).
+Proof. Admitted.
+
+(* end hide *)
+
+(* begin hide *)
+
+Lemma open_u_wrt_u_rec_degree_u_wrt_u :
+forall u2 u1 n1,
+  degree_u_wrt_u n1 u2 ->
+  open_u_wrt_u_rec n1 u1 u2 = u2.
+Proof. Admitted.
+
+Hint Resolve open_u_wrt_u_rec_degree_u_wrt_u : lngen.
+Hint Rewrite open_u_wrt_u_rec_degree_u_wrt_u using solve [auto] : lngen.
 
 (* end hide *)
 
@@ -1859,10 +2318,7 @@ Lemma open_u_wrt_t_rec_degree_u_wrt_t_mutual :
 (forall u1 t1 n1,
   degree_u_wrt_t n1 u1 ->
   open_u_wrt_t_rec n1 t1 u1 = u1).
-Proof.
-apply_mutual_ind u_mutind;
-default_simp.
-Qed.
+Proof. Admitted.
 
 (* end hide *)
 
@@ -1872,9 +2328,7 @@ Lemma open_u_wrt_t_rec_degree_u_wrt_t :
 forall u1 t1 n1,
   degree_u_wrt_t n1 u1 ->
   open_u_wrt_t_rec n1 t1 u1 = u1.
-Proof.
-pose proof open_u_wrt_t_rec_degree_u_wrt_t_mutual as H; intuition eauto.
-Qed.
+Proof. Admitted.
 
 Hint Resolve open_u_wrt_t_rec_degree_u_wrt_t : lngen.
 Hint Rewrite open_u_wrt_t_rec_degree_u_wrt_t using solve [auto] : lngen.
@@ -1885,20 +2339,25 @@ Lemma open_t_wrt_t_lc_t :
 forall t2 t1,
   lc_t t2 ->
   open_t_wrt_t t2 t1 = t2.
-Proof.
-unfold open_t_wrt_t; default_simp.
-Qed.
+Proof. Admitted.
 
 Hint Resolve open_t_wrt_t_lc_t : lngen.
 Hint Rewrite open_t_wrt_t_lc_t using solve [auto] : lngen.
+
+Lemma open_u_wrt_u_lc_u :
+forall u2 u1,
+  lc_u u2 ->
+  open_u_wrt_u u2 u1 = u2.
+Proof. Admitted.
+
+Hint Resolve open_u_wrt_u_lc_u : lngen.
+Hint Rewrite open_u_wrt_u_lc_u using solve [auto] : lngen.
 
 Lemma open_u_wrt_t_lc_u :
 forall u1 t1,
   lc_u u1 ->
   open_u_wrt_t u1 t1 = u1.
-Proof.
-unfold open_u_wrt_t; default_simp.
-Qed.
+Proof. Admitted.
 
 Hint Resolve open_u_wrt_t_lc_u : lngen.
 Hint Rewrite open_u_wrt_t_lc_u using solve [auto] : lngen.
@@ -1915,10 +2374,7 @@ Ltac default_autorewrite ::= autorewrite with lngen.
 Lemma tt_fv_t_close_t_wrt_t_rec_mutual :
 (forall t1 a1 n1,
   tt_fv_t (close_t_wrt_t_rec n1 a1 t1) [=] remove a1 (tt_fv_t t1)).
-Proof.
-apply_mutual_ind t_mutind;
-default_simp; fsetdec.
-Qed.
+Proof. Admitted.
 
 (* end hide *)
 
@@ -1927,9 +2383,7 @@ Qed.
 Lemma tt_fv_t_close_t_wrt_t_rec :
 forall t1 a1 n1,
   tt_fv_t (close_t_wrt_t_rec n1 a1 t1) [=] remove a1 (tt_fv_t t1).
-Proof.
-pose proof tt_fv_t_close_t_wrt_t_rec_mutual as H; intuition eauto.
-Qed.
+Proof. Admitted.
 
 Hint Resolve tt_fv_t_close_t_wrt_t_rec : lngen.
 Hint Rewrite tt_fv_t_close_t_wrt_t_rec using solve [auto] : lngen.
@@ -1938,13 +2392,73 @@ Hint Rewrite tt_fv_t_close_t_wrt_t_rec using solve [auto] : lngen.
 
 (* begin hide *)
 
+Lemma e_fv_u_close_u_wrt_u_rec_mutual :
+(forall u1 x1 n1,
+  e_fv_u (close_u_wrt_u_rec n1 x1 u1) [=] remove x1 (e_fv_u u1)).
+Proof. Admitted.
+
+(* end hide *)
+
+(* begin hide *)
+
+Lemma e_fv_u_close_u_wrt_u_rec :
+forall u1 x1 n1,
+  e_fv_u (close_u_wrt_u_rec n1 x1 u1) [=] remove x1 (e_fv_u u1).
+Proof. Admitted.
+
+Hint Resolve e_fv_u_close_u_wrt_u_rec : lngen.
+Hint Rewrite e_fv_u_close_u_wrt_u_rec using solve [auto] : lngen.
+
+(* end hide *)
+
+(* begin hide *)
+
+Lemma e_fv_u_close_u_wrt_t_rec_mutual :
+(forall u1 a1 n1,
+  e_fv_u (close_u_wrt_t_rec n1 a1 u1) [=] e_fv_u u1).
+Proof. Admitted.
+
+(* end hide *)
+
+(* begin hide *)
+
+Lemma e_fv_u_close_u_wrt_t_rec :
+forall u1 a1 n1,
+  e_fv_u (close_u_wrt_t_rec n1 a1 u1) [=] e_fv_u u1.
+Proof. Admitted.
+
+Hint Resolve e_fv_u_close_u_wrt_t_rec : lngen.
+Hint Rewrite e_fv_u_close_u_wrt_t_rec using solve [auto] : lngen.
+
+(* end hide *)
+
+(* begin hide *)
+
+Lemma tt_fv_u_close_u_wrt_u_rec_mutual :
+(forall u1 x1 n1,
+  tt_fv_u (close_u_wrt_u_rec n1 x1 u1) [=] tt_fv_u u1).
+Proof. Admitted.
+
+(* end hide *)
+
+(* begin hide *)
+
+Lemma tt_fv_u_close_u_wrt_u_rec :
+forall u1 x1 n1,
+  tt_fv_u (close_u_wrt_u_rec n1 x1 u1) [=] tt_fv_u u1.
+Proof. Admitted.
+
+Hint Resolve tt_fv_u_close_u_wrt_u_rec : lngen.
+Hint Rewrite tt_fv_u_close_u_wrt_u_rec using solve [auto] : lngen.
+
+(* end hide *)
+
+(* begin hide *)
+
 Lemma tt_fv_u_close_u_wrt_t_rec_mutual :
 (forall u1 a1 n1,
   tt_fv_u (close_u_wrt_t_rec n1 a1 u1) [=] remove a1 (tt_fv_u u1)).
-Proof.
-apply_mutual_ind u_mutind;
-default_simp; fsetdec.
-Qed.
+Proof. Admitted.
 
 (* end hide *)
 
@@ -1953,9 +2467,7 @@ Qed.
 Lemma tt_fv_u_close_u_wrt_t_rec :
 forall u1 a1 n1,
   tt_fv_u (close_u_wrt_t_rec n1 a1 u1) [=] remove a1 (tt_fv_u u1).
-Proof.
-pose proof tt_fv_u_close_u_wrt_t_rec_mutual as H; intuition eauto.
-Qed.
+Proof. Admitted.
 
 Hint Resolve tt_fv_u_close_u_wrt_t_rec : lngen.
 Hint Rewrite tt_fv_u_close_u_wrt_t_rec using solve [auto] : lngen.
@@ -1965,19 +2477,39 @@ Hint Rewrite tt_fv_u_close_u_wrt_t_rec using solve [auto] : lngen.
 Lemma tt_fv_t_close_t_wrt_t :
 forall t1 a1,
   tt_fv_t (close_t_wrt_t a1 t1) [=] remove a1 (tt_fv_t t1).
-Proof.
-unfold close_t_wrt_t; default_simp.
-Qed.
+Proof. Admitted.
 
 Hint Resolve tt_fv_t_close_t_wrt_t : lngen.
 Hint Rewrite tt_fv_t_close_t_wrt_t using solve [auto] : lngen.
 
+Lemma e_fv_u_close_u_wrt_u :
+forall u1 x1,
+  e_fv_u (close_u_wrt_u x1 u1) [=] remove x1 (e_fv_u u1).
+Proof. Admitted.
+
+Hint Resolve e_fv_u_close_u_wrt_u : lngen.
+Hint Rewrite e_fv_u_close_u_wrt_u using solve [auto] : lngen.
+
+Lemma e_fv_u_close_u_wrt_t :
+forall u1 a1,
+  e_fv_u (close_u_wrt_t a1 u1) [=] e_fv_u u1.
+Proof. Admitted.
+
+Hint Resolve e_fv_u_close_u_wrt_t : lngen.
+Hint Rewrite e_fv_u_close_u_wrt_t using solve [auto] : lngen.
+
+Lemma tt_fv_u_close_u_wrt_u :
+forall u1 x1,
+  tt_fv_u (close_u_wrt_u x1 u1) [=] tt_fv_u u1.
+Proof. Admitted.
+
+Hint Resolve tt_fv_u_close_u_wrt_u : lngen.
+Hint Rewrite tt_fv_u_close_u_wrt_u using solve [auto] : lngen.
+
 Lemma tt_fv_u_close_u_wrt_t :
 forall u1 a1,
   tt_fv_u (close_u_wrt_t a1 u1) [=] remove a1 (tt_fv_u u1).
-Proof.
-unfold close_u_wrt_t; default_simp.
-Qed.
+Proof. Admitted.
 
 Hint Resolve tt_fv_u_close_u_wrt_t : lngen.
 Hint Rewrite tt_fv_u_close_u_wrt_t using solve [auto] : lngen.
@@ -1987,10 +2519,7 @@ Hint Rewrite tt_fv_u_close_u_wrt_t using solve [auto] : lngen.
 Lemma tt_fv_t_open_t_wrt_t_rec_lower_mutual :
 (forall t1 t2 n1,
   tt_fv_t t1 [<=] tt_fv_t (open_t_wrt_t_rec n1 t2 t1)).
-Proof.
-apply_mutual_ind t_mutind;
-default_simp; fsetdec.
-Qed.
+Proof. Admitted.
 
 (* end hide *)
 
@@ -1999,11 +2528,69 @@ Qed.
 Lemma tt_fv_t_open_t_wrt_t_rec_lower :
 forall t1 t2 n1,
   tt_fv_t t1 [<=] tt_fv_t (open_t_wrt_t_rec n1 t2 t1).
-Proof.
-pose proof tt_fv_t_open_t_wrt_t_rec_lower_mutual as H; intuition eauto.
-Qed.
+Proof. Admitted.
 
 Hint Resolve tt_fv_t_open_t_wrt_t_rec_lower : lngen.
+
+(* end hide *)
+
+(* begin hide *)
+
+Lemma e_fv_u_open_u_wrt_u_rec_lower_mutual :
+(forall u1 u2 n1,
+  e_fv_u u1 [<=] e_fv_u (open_u_wrt_u_rec n1 u2 u1)).
+Proof. Admitted.
+
+(* end hide *)
+
+(* begin hide *)
+
+Lemma e_fv_u_open_u_wrt_u_rec_lower :
+forall u1 u2 n1,
+  e_fv_u u1 [<=] e_fv_u (open_u_wrt_u_rec n1 u2 u1).
+Proof. Admitted.
+
+Hint Resolve e_fv_u_open_u_wrt_u_rec_lower : lngen.
+
+(* end hide *)
+
+(* begin hide *)
+
+Lemma e_fv_u_open_u_wrt_t_rec_lower_mutual :
+(forall u1 t1 n1,
+  e_fv_u u1 [<=] e_fv_u (open_u_wrt_t_rec n1 t1 u1)).
+Proof. Admitted.
+
+(* end hide *)
+
+(* begin hide *)
+
+Lemma e_fv_u_open_u_wrt_t_rec_lower :
+forall u1 t1 n1,
+  e_fv_u u1 [<=] e_fv_u (open_u_wrt_t_rec n1 t1 u1).
+Proof. Admitted.
+
+Hint Resolve e_fv_u_open_u_wrt_t_rec_lower : lngen.
+
+(* end hide *)
+
+(* begin hide *)
+
+Lemma tt_fv_u_open_u_wrt_u_rec_lower_mutual :
+(forall u1 u2 n1,
+  tt_fv_u u1 [<=] tt_fv_u (open_u_wrt_u_rec n1 u2 u1)).
+Proof. Admitted.
+
+(* end hide *)
+
+(* begin hide *)
+
+Lemma tt_fv_u_open_u_wrt_u_rec_lower :
+forall u1 u2 n1,
+  tt_fv_u u1 [<=] tt_fv_u (open_u_wrt_u_rec n1 u2 u1).
+Proof. Admitted.
+
+Hint Resolve tt_fv_u_open_u_wrt_u_rec_lower : lngen.
 
 (* end hide *)
 
@@ -2012,10 +2599,7 @@ Hint Resolve tt_fv_t_open_t_wrt_t_rec_lower : lngen.
 Lemma tt_fv_u_open_u_wrt_t_rec_lower_mutual :
 (forall u1 t1 n1,
   tt_fv_u u1 [<=] tt_fv_u (open_u_wrt_t_rec n1 t1 u1)).
-Proof.
-apply_mutual_ind u_mutind;
-default_simp; fsetdec.
-Qed.
+Proof. Admitted.
 
 (* end hide *)
 
@@ -2024,9 +2608,7 @@ Qed.
 Lemma tt_fv_u_open_u_wrt_t_rec_lower :
 forall u1 t1 n1,
   tt_fv_u u1 [<=] tt_fv_u (open_u_wrt_t_rec n1 t1 u1).
-Proof.
-pose proof tt_fv_u_open_u_wrt_t_rec_lower_mutual as H; intuition eauto.
-Qed.
+Proof. Admitted.
 
 Hint Resolve tt_fv_u_open_u_wrt_t_rec_lower : lngen.
 
@@ -2035,18 +2617,35 @@ Hint Resolve tt_fv_u_open_u_wrt_t_rec_lower : lngen.
 Lemma tt_fv_t_open_t_wrt_t_lower :
 forall t1 t2,
   tt_fv_t t1 [<=] tt_fv_t (open_t_wrt_t t1 t2).
-Proof.
-unfold open_t_wrt_t; default_simp.
-Qed.
+Proof. Admitted.
 
 Hint Resolve tt_fv_t_open_t_wrt_t_lower : lngen.
+
+Lemma e_fv_u_open_u_wrt_u_lower :
+forall u1 u2,
+  e_fv_u u1 [<=] e_fv_u (open_u_wrt_u u1 u2).
+Proof. Admitted.
+
+Hint Resolve e_fv_u_open_u_wrt_u_lower : lngen.
+
+Lemma e_fv_u_open_u_wrt_t_lower :
+forall u1 t1,
+  e_fv_u u1 [<=] e_fv_u (open_u_wrt_t u1 t1).
+Proof. Admitted.
+
+Hint Resolve e_fv_u_open_u_wrt_t_lower : lngen.
+
+Lemma tt_fv_u_open_u_wrt_u_lower :
+forall u1 u2,
+  tt_fv_u u1 [<=] tt_fv_u (open_u_wrt_u u1 u2).
+Proof. Admitted.
+
+Hint Resolve tt_fv_u_open_u_wrt_u_lower : lngen.
 
 Lemma tt_fv_u_open_u_wrt_t_lower :
 forall u1 t1,
   tt_fv_u u1 [<=] tt_fv_u (open_u_wrt_t u1 t1).
-Proof.
-unfold open_u_wrt_t; default_simp.
-Qed.
+Proof. Admitted.
 
 Hint Resolve tt_fv_u_open_u_wrt_t_lower : lngen.
 
@@ -2055,10 +2654,7 @@ Hint Resolve tt_fv_u_open_u_wrt_t_lower : lngen.
 Lemma tt_fv_t_open_t_wrt_t_rec_upper_mutual :
 (forall t1 t2 n1,
   tt_fv_t (open_t_wrt_t_rec n1 t2 t1) [<=] tt_fv_t t2 `union` tt_fv_t t1).
-Proof.
-apply_mutual_ind t_mutind;
-default_simp; fsetdec.
-Qed.
+Proof. Admitted.
 
 (* end hide *)
 
@@ -2067,11 +2663,69 @@ Qed.
 Lemma tt_fv_t_open_t_wrt_t_rec_upper :
 forall t1 t2 n1,
   tt_fv_t (open_t_wrt_t_rec n1 t2 t1) [<=] tt_fv_t t2 `union` tt_fv_t t1.
-Proof.
-pose proof tt_fv_t_open_t_wrt_t_rec_upper_mutual as H; intuition eauto.
-Qed.
+Proof. Admitted.
 
 Hint Resolve tt_fv_t_open_t_wrt_t_rec_upper : lngen.
+
+(* end hide *)
+
+(* begin hide *)
+
+Lemma e_fv_u_open_u_wrt_u_rec_upper_mutual :
+(forall u1 u2 n1,
+  e_fv_u (open_u_wrt_u_rec n1 u2 u1) [<=] e_fv_u u2 `union` e_fv_u u1).
+Proof. Admitted.
+
+(* end hide *)
+
+(* begin hide *)
+
+Lemma e_fv_u_open_u_wrt_u_rec_upper :
+forall u1 u2 n1,
+  e_fv_u (open_u_wrt_u_rec n1 u2 u1) [<=] e_fv_u u2 `union` e_fv_u u1.
+Proof. Admitted.
+
+Hint Resolve e_fv_u_open_u_wrt_u_rec_upper : lngen.
+
+(* end hide *)
+
+(* begin hide *)
+
+Lemma e_fv_u_open_u_wrt_t_rec_upper_mutual :
+(forall u1 t1 n1,
+  e_fv_u (open_u_wrt_t_rec n1 t1 u1) [<=] e_fv_u u1).
+Proof. Admitted.
+
+(* end hide *)
+
+(* begin hide *)
+
+Lemma e_fv_u_open_u_wrt_t_rec_upper :
+forall u1 t1 n1,
+  e_fv_u (open_u_wrt_t_rec n1 t1 u1) [<=] e_fv_u u1.
+Proof. Admitted.
+
+Hint Resolve e_fv_u_open_u_wrt_t_rec_upper : lngen.
+
+(* end hide *)
+
+(* begin hide *)
+
+Lemma tt_fv_u_open_u_wrt_u_rec_upper_mutual :
+(forall u1 u2 n1,
+  tt_fv_u (open_u_wrt_u_rec n1 u2 u1) [<=] tt_fv_u u2 `union` tt_fv_u u1).
+Proof. Admitted.
+
+(* end hide *)
+
+(* begin hide *)
+
+Lemma tt_fv_u_open_u_wrt_u_rec_upper :
+forall u1 u2 n1,
+  tt_fv_u (open_u_wrt_u_rec n1 u2 u1) [<=] tt_fv_u u2 `union` tt_fv_u u1.
+Proof. Admitted.
+
+Hint Resolve tt_fv_u_open_u_wrt_u_rec_upper : lngen.
 
 (* end hide *)
 
@@ -2080,10 +2734,7 @@ Hint Resolve tt_fv_t_open_t_wrt_t_rec_upper : lngen.
 Lemma tt_fv_u_open_u_wrt_t_rec_upper_mutual :
 (forall u1 t1 n1,
   tt_fv_u (open_u_wrt_t_rec n1 t1 u1) [<=] tt_fv_t t1 `union` tt_fv_u u1).
-Proof.
-apply_mutual_ind u_mutind;
-default_simp; fsetdec.
-Qed.
+Proof. Admitted.
 
 (* end hide *)
 
@@ -2092,9 +2743,7 @@ Qed.
 Lemma tt_fv_u_open_u_wrt_t_rec_upper :
 forall u1 t1 n1,
   tt_fv_u (open_u_wrt_t_rec n1 t1 u1) [<=] tt_fv_t t1 `union` tt_fv_u u1.
-Proof.
-pose proof tt_fv_u_open_u_wrt_t_rec_upper_mutual as H; intuition eauto.
-Qed.
+Proof. Admitted.
 
 Hint Resolve tt_fv_u_open_u_wrt_t_rec_upper : lngen.
 
@@ -2103,18 +2752,35 @@ Hint Resolve tt_fv_u_open_u_wrt_t_rec_upper : lngen.
 Lemma tt_fv_t_open_t_wrt_t_upper :
 forall t1 t2,
   tt_fv_t (open_t_wrt_t t1 t2) [<=] tt_fv_t t2 `union` tt_fv_t t1.
-Proof.
-unfold open_t_wrt_t; default_simp.
-Qed.
+Proof. Admitted.
 
 Hint Resolve tt_fv_t_open_t_wrt_t_upper : lngen.
+
+Lemma e_fv_u_open_u_wrt_u_upper :
+forall u1 u2,
+  e_fv_u (open_u_wrt_u u1 u2) [<=] e_fv_u u2 `union` e_fv_u u1.
+Proof. Admitted.
+
+Hint Resolve e_fv_u_open_u_wrt_u_upper : lngen.
+
+Lemma e_fv_u_open_u_wrt_t_upper :
+forall u1 t1,
+  e_fv_u (open_u_wrt_t u1 t1) [<=] e_fv_u u1.
+Proof. Admitted.
+
+Hint Resolve e_fv_u_open_u_wrt_t_upper : lngen.
+
+Lemma tt_fv_u_open_u_wrt_u_upper :
+forall u1 u2,
+  tt_fv_u (open_u_wrt_u u1 u2) [<=] tt_fv_u u2 `union` tt_fv_u u1.
+Proof. Admitted.
+
+Hint Resolve tt_fv_u_open_u_wrt_u_upper : lngen.
 
 Lemma tt_fv_u_open_u_wrt_t_upper :
 forall u1 t1,
   tt_fv_u (open_u_wrt_t u1 t1) [<=] tt_fv_t t1 `union` tt_fv_u u1.
-Proof.
-unfold open_u_wrt_t; default_simp.
-Qed.
+Proof. Admitted.
 
 Hint Resolve tt_fv_u_open_u_wrt_t_upper : lngen.
 
@@ -2124,10 +2790,7 @@ Lemma tt_fv_t_t_subst_t_fresh_mutual :
 (forall t1 t2 a1,
   a1 `notin` tt_fv_t t1 ->
   tt_fv_t (t_subst_t t2 a1 t1) [=] tt_fv_t t1).
-Proof.
-apply_mutual_ind t_mutind;
-default_simp; fsetdec.
-Qed.
+Proof. Admitted.
 
 (* end hide *)
 
@@ -2135,12 +2798,46 @@ Lemma tt_fv_t_t_subst_t_fresh :
 forall t1 t2 a1,
   a1 `notin` tt_fv_t t1 ->
   tt_fv_t (t_subst_t t2 a1 t1) [=] tt_fv_t t1.
-Proof.
-pose proof tt_fv_t_t_subst_t_fresh_mutual as H; intuition eauto.
-Qed.
+Proof. Admitted.
 
 Hint Resolve tt_fv_t_t_subst_t_fresh : lngen.
 Hint Rewrite tt_fv_t_t_subst_t_fresh using solve [auto] : lngen.
+
+(* begin hide *)
+
+Lemma e_fv_u_e_subst_u_fresh_mutual :
+(forall u1 u2 x1,
+  x1 `notin` e_fv_u u1 ->
+  e_fv_u (e_subst_u u2 x1 u1) [=] e_fv_u u1).
+Proof. Admitted.
+
+(* end hide *)
+
+Lemma e_fv_u_e_subst_u_fresh :
+forall u1 u2 x1,
+  x1 `notin` e_fv_u u1 ->
+  e_fv_u (e_subst_u u2 x1 u1) [=] e_fv_u u1.
+Proof. Admitted.
+
+Hint Resolve e_fv_u_e_subst_u_fresh : lngen.
+Hint Rewrite e_fv_u_e_subst_u_fresh using solve [auto] : lngen.
+
+(* begin hide *)
+
+Lemma tt_fv_u_e_subst_u_fresh_mutual :
+(forall u1 t1 a1,
+  e_fv_u (t_subst_u t1 a1 u1) [=] e_fv_u u1).
+Proof. Admitted.
+
+(* end hide *)
+
+Lemma tt_fv_u_e_subst_u_fresh :
+forall u1 t1 a1,
+  e_fv_u (t_subst_u t1 a1 u1) [=] e_fv_u u1.
+Proof. Admitted.
+
+Hint Resolve tt_fv_u_e_subst_u_fresh : lngen.
+Hint Rewrite tt_fv_u_e_subst_u_fresh using solve [auto] : lngen.
 
 (* begin hide *)
 
@@ -2148,10 +2845,7 @@ Lemma tt_fv_u_t_subst_u_fresh_mutual :
 (forall u1 t1 a1,
   a1 `notin` tt_fv_u u1 ->
   tt_fv_u (t_subst_u t1 a1 u1) [=] tt_fv_u u1).
-Proof.
-apply_mutual_ind u_mutind;
-default_simp; fsetdec.
-Qed.
+Proof. Admitted.
 
 (* end hide *)
 
@@ -2159,9 +2853,7 @@ Lemma tt_fv_u_t_subst_u_fresh :
 forall u1 t1 a1,
   a1 `notin` tt_fv_u u1 ->
   tt_fv_u (t_subst_u t1 a1 u1) [=] tt_fv_u u1.
-Proof.
-pose proof tt_fv_u_t_subst_u_fresh_mutual as H; intuition eauto.
-Qed.
+Proof. Admitted.
 
 Hint Resolve tt_fv_u_t_subst_u_fresh : lngen.
 Hint Rewrite tt_fv_u_t_subst_u_fresh using solve [auto] : lngen.
@@ -2171,40 +2863,78 @@ Hint Rewrite tt_fv_u_t_subst_u_fresh using solve [auto] : lngen.
 Lemma tt_fv_t_t_subst_t_lower_mutual :
 (forall t1 t2 a1,
   remove a1 (tt_fv_t t1) [<=] tt_fv_t (t_subst_t t2 a1 t1)).
-Proof.
-apply_mutual_ind t_mutind;
-default_simp; fsetdec.
-Qed.
+Proof. Admitted.
 
 (* end hide *)
 
 Lemma tt_fv_t_t_subst_t_lower :
 forall t1 t2 a1,
   remove a1 (tt_fv_t t1) [<=] tt_fv_t (t_subst_t t2 a1 t1).
-Proof.
-pose proof tt_fv_t_t_subst_t_lower_mutual as H; intuition eauto.
-Qed.
+Proof. Admitted.
 
 Hint Resolve tt_fv_t_t_subst_t_lower : lngen.
+
+(* begin hide *)
+
+Lemma e_fv_u_e_subst_u_lower_mutual :
+(forall u1 u2 x1,
+  remove x1 (e_fv_u u1) [<=] e_fv_u (e_subst_u u2 x1 u1)).
+Proof. Admitted.
+
+(* end hide *)
+
+Lemma e_fv_u_e_subst_u_lower :
+forall u1 u2 x1,
+  remove x1 (e_fv_u u1) [<=] e_fv_u (e_subst_u u2 x1 u1).
+Proof. Admitted.
+
+Hint Resolve e_fv_u_e_subst_u_lower : lngen.
+
+(* begin hide *)
+
+Lemma e_fv_u_t_subst_u_lower_mutual :
+(forall u1 t1 a1,
+  e_fv_u u1 [<=] e_fv_u (t_subst_u t1 a1 u1)).
+Proof. Admitted.
+
+(* end hide *)
+
+Lemma e_fv_u_t_subst_u_lower :
+forall u1 t1 a1,
+  e_fv_u u1 [<=] e_fv_u (t_subst_u t1 a1 u1).
+Proof. Admitted.
+
+Hint Resolve e_fv_u_t_subst_u_lower : lngen.
+
+(* begin hide *)
+
+Lemma tt_fv_u_e_subst_u_lower_mutual :
+(forall u1 u2 x1,
+  tt_fv_u u1 [<=] tt_fv_u (e_subst_u u2 x1 u1)).
+Proof. Admitted.
+
+(* end hide *)
+
+Lemma tt_fv_u_e_subst_u_lower :
+forall u1 u2 x1,
+  tt_fv_u u1 [<=] tt_fv_u (e_subst_u u2 x1 u1).
+Proof. Admitted.
+
+Hint Resolve tt_fv_u_e_subst_u_lower : lngen.
 
 (* begin hide *)
 
 Lemma tt_fv_u_t_subst_u_lower_mutual :
 (forall u1 t1 a1,
   remove a1 (tt_fv_u u1) [<=] tt_fv_u (t_subst_u t1 a1 u1)).
-Proof.
-apply_mutual_ind u_mutind;
-default_simp; fsetdec.
-Qed.
+Proof. Admitted.
 
 (* end hide *)
 
 Lemma tt_fv_u_t_subst_u_lower :
 forall u1 t1 a1,
   remove a1 (tt_fv_u u1) [<=] tt_fv_u (t_subst_u t1 a1 u1).
-Proof.
-pose proof tt_fv_u_t_subst_u_lower_mutual as H; intuition eauto.
-Qed.
+Proof. Admitted.
 
 Hint Resolve tt_fv_u_t_subst_u_lower : lngen.
 
@@ -2215,10 +2945,7 @@ Lemma tt_fv_t_t_subst_t_notin_mutual :
   a2 `notin` tt_fv_t t1 ->
   a2 `notin` tt_fv_t t2 ->
   a2 `notin` tt_fv_t (t_subst_t t2 a1 t1)).
-Proof.
-apply_mutual_ind t_mutind;
-default_simp; fsetdec.
-Qed.
+Proof. Admitted.
 
 (* end hide *)
 
@@ -2227,11 +2954,67 @@ forall t1 t2 a1 a2,
   a2 `notin` tt_fv_t t1 ->
   a2 `notin` tt_fv_t t2 ->
   a2 `notin` tt_fv_t (t_subst_t t2 a1 t1).
-Proof.
-pose proof tt_fv_t_t_subst_t_notin_mutual as H; intuition eauto.
-Qed.
+Proof. Admitted.
 
 Hint Resolve tt_fv_t_t_subst_t_notin : lngen.
+
+(* begin hide *)
+
+Lemma e_fv_u_e_subst_u_notin_mutual :
+(forall u1 u2 x1 x2,
+  x2 `notin` e_fv_u u1 ->
+  x2 `notin` e_fv_u u2 ->
+  x2 `notin` e_fv_u (e_subst_u u2 x1 u1)).
+Proof. Admitted.
+
+(* end hide *)
+
+Lemma e_fv_u_e_subst_u_notin :
+forall u1 u2 x1 x2,
+  x2 `notin` e_fv_u u1 ->
+  x2 `notin` e_fv_u u2 ->
+  x2 `notin` e_fv_u (e_subst_u u2 x1 u1).
+Proof. Admitted.
+
+Hint Resolve e_fv_u_e_subst_u_notin : lngen.
+
+(* begin hide *)
+
+Lemma e_fv_u_t_subst_u_notin_mutual :
+(forall u1 t1 a1 x1,
+  x1 `notin` e_fv_u u1 ->
+  x1 `notin` e_fv_u (t_subst_u t1 a1 u1)).
+Proof. Admitted.
+
+(* end hide *)
+
+Lemma e_fv_u_t_subst_u_notin :
+forall u1 t1 a1 x1,
+  x1 `notin` e_fv_u u1 ->
+  x1 `notin` e_fv_u (t_subst_u t1 a1 u1).
+Proof. Admitted.
+
+Hint Resolve e_fv_u_t_subst_u_notin : lngen.
+
+(* begin hide *)
+
+Lemma tt_fv_u_e_subst_u_notin_mutual :
+(forall u1 u2 x1 a1,
+  a1 `notin` tt_fv_u u1 ->
+  a1 `notin` tt_fv_u u2 ->
+  a1 `notin` tt_fv_u (e_subst_u u2 x1 u1)).
+Proof. Admitted.
+
+(* end hide *)
+
+Lemma tt_fv_u_e_subst_u_notin :
+forall u1 u2 x1 a1,
+  a1 `notin` tt_fv_u u1 ->
+  a1 `notin` tt_fv_u u2 ->
+  a1 `notin` tt_fv_u (e_subst_u u2 x1 u1).
+Proof. Admitted.
+
+Hint Resolve tt_fv_u_e_subst_u_notin : lngen.
 
 (* begin hide *)
 
@@ -2240,10 +3023,7 @@ Lemma tt_fv_u_t_subst_u_notin_mutual :
   a2 `notin` tt_fv_u u1 ->
   a2 `notin` tt_fv_t t1 ->
   a2 `notin` tt_fv_u (t_subst_u t1 a1 u1)).
-Proof.
-apply_mutual_ind u_mutind;
-default_simp; fsetdec.
-Qed.
+Proof. Admitted.
 
 (* end hide *)
 
@@ -2252,9 +3032,7 @@ forall u1 t1 a1 a2,
   a2 `notin` tt_fv_u u1 ->
   a2 `notin` tt_fv_t t1 ->
   a2 `notin` tt_fv_u (t_subst_u t1 a1 u1).
-Proof.
-pose proof tt_fv_u_t_subst_u_notin_mutual as H; intuition eauto.
-Qed.
+Proof. Admitted.
 
 Hint Resolve tt_fv_u_t_subst_u_notin : lngen.
 
@@ -2263,40 +3041,78 @@ Hint Resolve tt_fv_u_t_subst_u_notin : lngen.
 Lemma tt_fv_t_t_subst_t_upper_mutual :
 (forall t1 t2 a1,
   tt_fv_t (t_subst_t t2 a1 t1) [<=] tt_fv_t t2 `union` remove a1 (tt_fv_t t1)).
-Proof.
-apply_mutual_ind t_mutind;
-default_simp; fsetdec.
-Qed.
+Proof. Admitted.
 
 (* end hide *)
 
 Lemma tt_fv_t_t_subst_t_upper :
 forall t1 t2 a1,
   tt_fv_t (t_subst_t t2 a1 t1) [<=] tt_fv_t t2 `union` remove a1 (tt_fv_t t1).
-Proof.
-pose proof tt_fv_t_t_subst_t_upper_mutual as H; intuition eauto.
-Qed.
+Proof. Admitted.
 
 Hint Resolve tt_fv_t_t_subst_t_upper : lngen.
+
+(* begin hide *)
+
+Lemma e_fv_u_e_subst_u_upper_mutual :
+(forall u1 u2 x1,
+  e_fv_u (e_subst_u u2 x1 u1) [<=] e_fv_u u2 `union` remove x1 (e_fv_u u1)).
+Proof. Admitted.
+
+(* end hide *)
+
+Lemma e_fv_u_e_subst_u_upper :
+forall u1 u2 x1,
+  e_fv_u (e_subst_u u2 x1 u1) [<=] e_fv_u u2 `union` remove x1 (e_fv_u u1).
+Proof. Admitted.
+
+Hint Resolve e_fv_u_e_subst_u_upper : lngen.
+
+(* begin hide *)
+
+Lemma e_fv_u_t_subst_u_upper_mutual :
+(forall u1 t1 a1,
+  e_fv_u (t_subst_u t1 a1 u1) [<=] e_fv_u u1).
+Proof. Admitted.
+
+(* end hide *)
+
+Lemma e_fv_u_t_subst_u_upper :
+forall u1 t1 a1,
+  e_fv_u (t_subst_u t1 a1 u1) [<=] e_fv_u u1.
+Proof. Admitted.
+
+Hint Resolve e_fv_u_t_subst_u_upper : lngen.
+
+(* begin hide *)
+
+Lemma tt_fv_u_e_subst_u_upper_mutual :
+(forall u1 u2 x1,
+  tt_fv_u (e_subst_u u2 x1 u1) [<=] tt_fv_u u2 `union` tt_fv_u u1).
+Proof. Admitted.
+
+(* end hide *)
+
+Lemma tt_fv_u_e_subst_u_upper :
+forall u1 u2 x1,
+  tt_fv_u (e_subst_u u2 x1 u1) [<=] tt_fv_u u2 `union` tt_fv_u u1.
+Proof. Admitted.
+
+Hint Resolve tt_fv_u_e_subst_u_upper : lngen.
 
 (* begin hide *)
 
 Lemma tt_fv_u_t_subst_u_upper_mutual :
 (forall u1 t1 a1,
   tt_fv_u (t_subst_u t1 a1 u1) [<=] tt_fv_t t1 `union` remove a1 (tt_fv_u u1)).
-Proof.
-apply_mutual_ind u_mutind;
-default_simp; fsetdec.
-Qed.
+Proof. Admitted.
 
 (* end hide *)
 
 Lemma tt_fv_u_t_subst_u_upper :
 forall u1 t1 a1,
   tt_fv_u (t_subst_u t1 a1 u1) [<=] tt_fv_t t1 `union` remove a1 (tt_fv_u u1).
-Proof.
-pose proof tt_fv_u_t_subst_u_upper_mutual as H; intuition eauto.
-Qed.
+Proof. Admitted.
 
 Hint Resolve tt_fv_u_t_subst_u_upper : lngen.
 
@@ -2315,10 +3131,7 @@ Lemma t_subst_t_close_t_wrt_t_rec_mutual :
   a1 <> a2 ->
   a2 `notin` tt_fv_t t1 ->
   t_subst_t t1 a1 (close_t_wrt_t_rec n1 a2 t2) = close_t_wrt_t_rec n1 a2 (t_subst_t t1 a1 t2)).
-Proof.
-apply_mutual_ind t_mutind;
-default_simp.
-Qed.
+Proof. Admitted.
 
 (* end hide *)
 
@@ -2328,11 +3141,67 @@ forall t2 t1 a1 a2 n1,
   a1 <> a2 ->
   a2 `notin` tt_fv_t t1 ->
   t_subst_t t1 a1 (close_t_wrt_t_rec n1 a2 t2) = close_t_wrt_t_rec n1 a2 (t_subst_t t1 a1 t2).
-Proof.
-pose proof t_subst_t_close_t_wrt_t_rec_mutual as H; intuition eauto.
-Qed.
+Proof. Admitted.
 
 Hint Resolve t_subst_t_close_t_wrt_t_rec : lngen.
+
+(* begin hide *)
+
+Lemma e_subst_u_close_u_wrt_u_rec_mutual :
+(forall u2 u1 x1 x2 n1,
+  degree_u_wrt_u n1 u1 ->
+  x1 <> x2 ->
+  x2 `notin` e_fv_u u1 ->
+  e_subst_u u1 x1 (close_u_wrt_u_rec n1 x2 u2) = close_u_wrt_u_rec n1 x2 (e_subst_u u1 x1 u2)).
+Proof. Admitted.
+
+(* end hide *)
+
+Lemma e_subst_u_close_u_wrt_u_rec :
+forall u2 u1 x1 x2 n1,
+  degree_u_wrt_u n1 u1 ->
+  x1 <> x2 ->
+  x2 `notin` e_fv_u u1 ->
+  e_subst_u u1 x1 (close_u_wrt_u_rec n1 x2 u2) = close_u_wrt_u_rec n1 x2 (e_subst_u u1 x1 u2).
+Proof. Admitted.
+
+Hint Resolve e_subst_u_close_u_wrt_u_rec : lngen.
+
+(* begin hide *)
+
+Lemma e_subst_u_close_u_wrt_t_rec_mutual :
+(forall u2 u1 a1 x1 n1,
+  degree_u_wrt_t n1 u1 ->
+  x1 `notin` tt_fv_u u1 ->
+  e_subst_u u1 a1 (close_u_wrt_t_rec n1 x1 u2) = close_u_wrt_t_rec n1 x1 (e_subst_u u1 a1 u2)).
+Proof. Admitted.
+
+(* end hide *)
+
+Lemma e_subst_u_close_u_wrt_t_rec :
+forall u2 u1 a1 x1 n1,
+  degree_u_wrt_t n1 u1 ->
+  x1 `notin` tt_fv_u u1 ->
+  e_subst_u u1 a1 (close_u_wrt_t_rec n1 x1 u2) = close_u_wrt_t_rec n1 x1 (e_subst_u u1 a1 u2).
+Proof. Admitted.
+
+Hint Resolve e_subst_u_close_u_wrt_t_rec : lngen.
+
+(* begin hide *)
+
+Lemma t_subst_u_close_u_wrt_u_rec_mutual :
+(forall u1 t1 x1 a1 n1,
+  t_subst_u t1 x1 (close_u_wrt_u_rec n1 a1 u1) = close_u_wrt_u_rec n1 a1 (t_subst_u t1 x1 u1)).
+Proof. Admitted.
+
+(* end hide *)
+
+Lemma t_subst_u_close_u_wrt_u_rec :
+forall u1 t1 x1 a1 n1,
+  t_subst_u t1 x1 (close_u_wrt_u_rec n1 a1 u1) = close_u_wrt_u_rec n1 a1 (t_subst_u t1 x1 u1).
+Proof. Admitted.
+
+Hint Resolve t_subst_u_close_u_wrt_u_rec : lngen.
 
 (* begin hide *)
 
@@ -2342,10 +3211,7 @@ Lemma t_subst_u_close_u_wrt_t_rec_mutual :
   a1 <> a2 ->
   a2 `notin` tt_fv_t t1 ->
   t_subst_u t1 a1 (close_u_wrt_t_rec n1 a2 u1) = close_u_wrt_t_rec n1 a2 (t_subst_u t1 a1 u1)).
-Proof.
-apply_mutual_ind u_mutind;
-default_simp.
-Qed.
+Proof. Admitted.
 
 (* end hide *)
 
@@ -2355,9 +3221,7 @@ forall u1 t1 a1 a2 n1,
   a1 <> a2 ->
   a2 `notin` tt_fv_t t1 ->
   t_subst_u t1 a1 (close_u_wrt_t_rec n1 a2 u1) = close_u_wrt_t_rec n1 a2 (t_subst_u t1 a1 u1).
-Proof.
-pose proof t_subst_u_close_u_wrt_t_rec_mutual as H; intuition eauto.
-Qed.
+Proof. Admitted.
 
 Hint Resolve t_subst_u_close_u_wrt_t_rec : lngen.
 
@@ -2366,20 +3230,40 @@ forall t2 t1 a1 a2,
   lc_t t1 ->  a1 <> a2 ->
   a2 `notin` tt_fv_t t1 ->
   t_subst_t t1 a1 (close_t_wrt_t a2 t2) = close_t_wrt_t a2 (t_subst_t t1 a1 t2).
-Proof.
-unfold close_t_wrt_t; default_simp.
-Qed.
+Proof. Admitted.
 
 Hint Resolve t_subst_t_close_t_wrt_t : lngen.
+
+Lemma e_subst_u_close_u_wrt_u :
+forall u2 u1 x1 x2,
+  lc_u u1 ->  x1 <> x2 ->
+  x2 `notin` e_fv_u u1 ->
+  e_subst_u u1 x1 (close_u_wrt_u x2 u2) = close_u_wrt_u x2 (e_subst_u u1 x1 u2).
+Proof. Admitted.
+
+Hint Resolve e_subst_u_close_u_wrt_u : lngen.
+
+Lemma e_subst_u_close_u_wrt_t :
+forall u2 u1 a1 x1,
+  lc_u u1 ->  x1 `notin` tt_fv_u u1 ->
+  e_subst_u u1 a1 (close_u_wrt_t x1 u2) = close_u_wrt_t x1 (e_subst_u u1 a1 u2).
+Proof. Admitted.
+
+Hint Resolve e_subst_u_close_u_wrt_t : lngen.
+
+Lemma t_subst_u_close_u_wrt_u :
+forall u1 t1 x1 a1,
+  lc_t t1 ->  t_subst_u t1 x1 (close_u_wrt_u a1 u1) = close_u_wrt_u a1 (t_subst_u t1 x1 u1).
+Proof. Admitted.
+
+Hint Resolve t_subst_u_close_u_wrt_u : lngen.
 
 Lemma t_subst_u_close_u_wrt_t :
 forall u1 t1 a1 a2,
   lc_t t1 ->  a1 <> a2 ->
   a2 `notin` tt_fv_t t1 ->
   t_subst_u t1 a1 (close_u_wrt_t a2 u1) = close_u_wrt_t a2 (t_subst_u t1 a1 u1).
-Proof.
-unfold close_u_wrt_t; default_simp.
-Qed.
+Proof. Admitted.
 
 Hint Resolve t_subst_u_close_u_wrt_t : lngen.
 
@@ -2390,10 +3274,7 @@ Lemma t_subst_t_degree_t_wrt_t_mutual :
   degree_t_wrt_t n1 t1 ->
   degree_t_wrt_t n1 t2 ->
   degree_t_wrt_t n1 (t_subst_t t2 a1 t1)).
-Proof.
-apply_mutual_ind t_mutind;
-default_simp.
-Qed.
+Proof. Admitted.
 
 (* end hide *)
 
@@ -2402,11 +3283,67 @@ forall t1 t2 a1 n1,
   degree_t_wrt_t n1 t1 ->
   degree_t_wrt_t n1 t2 ->
   degree_t_wrt_t n1 (t_subst_t t2 a1 t1).
-Proof.
-pose proof t_subst_t_degree_t_wrt_t_mutual as H; intuition eauto.
-Qed.
+Proof. Admitted.
 
 Hint Resolve t_subst_t_degree_t_wrt_t : lngen.
+
+(* begin hide *)
+
+Lemma e_subst_u_degree_u_wrt_u_mutual :
+(forall u1 u2 x1 n1,
+  degree_u_wrt_u n1 u1 ->
+  degree_u_wrt_u n1 u2 ->
+  degree_u_wrt_u n1 (e_subst_u u2 x1 u1)).
+Proof. Admitted.
+
+(* end hide *)
+
+Lemma e_subst_u_degree_u_wrt_u :
+forall u1 u2 x1 n1,
+  degree_u_wrt_u n1 u1 ->
+  degree_u_wrt_u n1 u2 ->
+  degree_u_wrt_u n1 (e_subst_u u2 x1 u1).
+Proof. Admitted.
+
+Hint Resolve e_subst_u_degree_u_wrt_u : lngen.
+
+(* begin hide *)
+
+Lemma e_subst_u_degree_u_wrt_t_mutual :
+(forall u1 u2 x1 n1,
+  degree_u_wrt_t n1 u1 ->
+  degree_u_wrt_t n1 u2 ->
+  degree_u_wrt_t n1 (e_subst_u u2 x1 u1)).
+Proof. Admitted.
+
+(* end hide *)
+
+Lemma e_subst_u_degree_u_wrt_t :
+forall u1 u2 x1 n1,
+  degree_u_wrt_t n1 u1 ->
+  degree_u_wrt_t n1 u2 ->
+  degree_u_wrt_t n1 (e_subst_u u2 x1 u1).
+Proof. Admitted.
+
+Hint Resolve e_subst_u_degree_u_wrt_t : lngen.
+
+(* begin hide *)
+
+Lemma t_subst_u_degree_u_wrt_u_mutual :
+(forall u1 t1 a1 n1,
+  degree_u_wrt_u n1 u1 ->
+  degree_u_wrt_u n1 (t_subst_u t1 a1 u1)).
+Proof. Admitted.
+
+(* end hide *)
+
+Lemma t_subst_u_degree_u_wrt_u :
+forall u1 t1 a1 n1,
+  degree_u_wrt_u n1 u1 ->
+  degree_u_wrt_u n1 (t_subst_u t1 a1 u1).
+Proof. Admitted.
+
+Hint Resolve t_subst_u_degree_u_wrt_u : lngen.
 
 (* begin hide *)
 
@@ -2415,10 +3352,7 @@ Lemma t_subst_u_degree_u_wrt_t_mutual :
   degree_u_wrt_t n1 u1 ->
   degree_t_wrt_t n1 t1 ->
   degree_u_wrt_t n1 (t_subst_u t1 a1 u1)).
-Proof.
-apply_mutual_ind u_mutind;
-default_simp.
-Qed.
+Proof. Admitted.
 
 (* end hide *)
 
@@ -2427,9 +3361,7 @@ forall u1 t1 a1 n1,
   degree_u_wrt_t n1 u1 ->
   degree_t_wrt_t n1 t1 ->
   degree_u_wrt_t n1 (t_subst_u t1 a1 u1).
-Proof.
-pose proof t_subst_u_degree_u_wrt_t_mutual as H; intuition eauto.
-Qed.
+Proof. Admitted.
 
 Hint Resolve t_subst_u_degree_u_wrt_t : lngen.
 
@@ -2439,10 +3371,7 @@ Lemma t_subst_t_fresh_eq_mutual :
 (forall t2 t1 a1,
   a1 `notin` tt_fv_t t2 ->
   t_subst_t t1 a1 t2 = t2).
-Proof.
-apply_mutual_ind t_mutind;
-default_simp.
-Qed.
+Proof. Admitted.
 
 (* end hide *)
 
@@ -2450,12 +3379,29 @@ Lemma t_subst_t_fresh_eq :
 forall t2 t1 a1,
   a1 `notin` tt_fv_t t2 ->
   t_subst_t t1 a1 t2 = t2.
-Proof.
-pose proof t_subst_t_fresh_eq_mutual as H; intuition eauto.
-Qed.
+Proof. Admitted.
 
 Hint Resolve t_subst_t_fresh_eq : lngen.
 Hint Rewrite t_subst_t_fresh_eq using solve [auto] : lngen.
+
+(* begin hide *)
+
+Lemma e_subst_u_fresh_eq_mutual :
+(forall u2 u1 x1,
+  x1 `notin` e_fv_u u2 ->
+  e_subst_u u1 x1 u2 = u2).
+Proof. Admitted.
+
+(* end hide *)
+
+Lemma e_subst_u_fresh_eq :
+forall u2 u1 x1,
+  x1 `notin` e_fv_u u2 ->
+  e_subst_u u1 x1 u2 = u2.
+Proof. Admitted.
+
+Hint Resolve e_subst_u_fresh_eq : lngen.
+Hint Rewrite e_subst_u_fresh_eq using solve [auto] : lngen.
 
 (* begin hide *)
 
@@ -2463,10 +3409,7 @@ Lemma t_subst_u_fresh_eq_mutual :
 (forall u1 t1 a1,
   a1 `notin` tt_fv_u u1 ->
   t_subst_u t1 a1 u1 = u1).
-Proof.
-apply_mutual_ind u_mutind;
-default_simp.
-Qed.
+Proof. Admitted.
 
 (* end hide *)
 
@@ -2474,9 +3417,7 @@ Lemma t_subst_u_fresh_eq :
 forall u1 t1 a1,
   a1 `notin` tt_fv_u u1 ->
   t_subst_u t1 a1 u1 = u1.
-Proof.
-pose proof t_subst_u_fresh_eq_mutual as H; intuition eauto.
-Qed.
+Proof. Admitted.
 
 Hint Resolve t_subst_u_fresh_eq : lngen.
 Hint Rewrite t_subst_u_fresh_eq using solve [auto] : lngen.
@@ -2487,10 +3428,7 @@ Lemma t_subst_t_fresh_same_mutual :
 (forall t2 t1 a1,
   a1 `notin` tt_fv_t t1 ->
   a1 `notin` tt_fv_t (t_subst_t t1 a1 t2)).
-Proof.
-apply_mutual_ind t_mutind;
-default_simp.
-Qed.
+Proof. Admitted.
 
 (* end hide *)
 
@@ -2498,11 +3436,27 @@ Lemma t_subst_t_fresh_same :
 forall t2 t1 a1,
   a1 `notin` tt_fv_t t1 ->
   a1 `notin` tt_fv_t (t_subst_t t1 a1 t2).
-Proof.
-pose proof t_subst_t_fresh_same_mutual as H; intuition eauto.
-Qed.
+Proof. Admitted.
 
 Hint Resolve t_subst_t_fresh_same : lngen.
+
+(* begin hide *)
+
+Lemma e_subst_u_fresh_same_mutual :
+(forall u2 u1 x1,
+  x1 `notin` e_fv_u u1 ->
+  x1 `notin` e_fv_u (e_subst_u u1 x1 u2)).
+Proof. Admitted.
+
+(* end hide *)
+
+Lemma e_subst_u_fresh_same :
+forall u2 u1 x1,
+  x1 `notin` e_fv_u u1 ->
+  x1 `notin` e_fv_u (e_subst_u u1 x1 u2).
+Proof. Admitted.
+
+Hint Resolve e_subst_u_fresh_same : lngen.
 
 (* begin hide *)
 
@@ -2510,10 +3464,7 @@ Lemma t_subst_u_fresh_same_mutual :
 (forall u1 t1 a1,
   a1 `notin` tt_fv_t t1 ->
   a1 `notin` tt_fv_u (t_subst_u t1 a1 u1)).
-Proof.
-apply_mutual_ind u_mutind;
-default_simp.
-Qed.
+Proof. Admitted.
 
 (* end hide *)
 
@@ -2521,9 +3472,7 @@ Lemma t_subst_u_fresh_same :
 forall u1 t1 a1,
   a1 `notin` tt_fv_t t1 ->
   a1 `notin` tt_fv_u (t_subst_u t1 a1 u1).
-Proof.
-pose proof t_subst_u_fresh_same_mutual as H; intuition eauto.
-Qed.
+Proof. Admitted.
 
 Hint Resolve t_subst_u_fresh_same : lngen.
 
@@ -2534,10 +3483,7 @@ Lemma t_subst_t_fresh_mutual :
   a1 `notin` tt_fv_t t2 ->
   a1 `notin` tt_fv_t t1 ->
   a1 `notin` tt_fv_t (t_subst_t t1 a2 t2)).
-Proof.
-apply_mutual_ind t_mutind;
-default_simp.
-Qed.
+Proof. Admitted.
 
 (* end hide *)
 
@@ -2546,11 +3492,29 @@ forall t2 t1 a1 a2,
   a1 `notin` tt_fv_t t2 ->
   a1 `notin` tt_fv_t t1 ->
   a1 `notin` tt_fv_t (t_subst_t t1 a2 t2).
-Proof.
-pose proof t_subst_t_fresh_mutual as H; intuition eauto.
-Qed.
+Proof. Admitted.
 
 Hint Resolve t_subst_t_fresh : lngen.
+
+(* begin hide *)
+
+Lemma e_subst_u_fresh_mutual :
+(forall u2 u1 x1 x2,
+  x1 `notin` e_fv_u u2 ->
+  x1 `notin` e_fv_u u1 ->
+  x1 `notin` e_fv_u (e_subst_u u1 x2 u2)).
+Proof. Admitted.
+
+(* end hide *)
+
+Lemma e_subst_u_fresh :
+forall u2 u1 x1 x2,
+  x1 `notin` e_fv_u u2 ->
+  x1 `notin` e_fv_u u1 ->
+  x1 `notin` e_fv_u (e_subst_u u1 x2 u2).
+Proof. Admitted.
+
+Hint Resolve e_subst_u_fresh : lngen.
 
 (* begin hide *)
 
@@ -2559,10 +3523,7 @@ Lemma t_subst_u_fresh_mutual :
   a1 `notin` tt_fv_u u1 ->
   a1 `notin` tt_fv_t t1 ->
   a1 `notin` tt_fv_u (t_subst_u t1 a2 u1)).
-Proof.
-apply_mutual_ind u_mutind;
-default_simp.
-Qed.
+Proof. Admitted.
 
 (* end hide *)
 
@@ -2571,9 +3532,7 @@ forall u1 t1 a1 a2,
   a1 `notin` tt_fv_u u1 ->
   a1 `notin` tt_fv_t t1 ->
   a1 `notin` tt_fv_u (t_subst_u t1 a2 u1).
-Proof.
-pose proof t_subst_u_fresh_mutual as H; intuition eauto.
-Qed.
+Proof. Admitted.
 
 Hint Resolve t_subst_u_fresh : lngen.
 
@@ -2582,20 +3541,25 @@ forall t1 t2 a1,
   lc_t t1 ->
   lc_t t2 ->
   lc_t (t_subst_t t2 a1 t1).
-Proof.
-default_simp.
-Qed.
+Proof. Admitted.
 
 Hint Resolve t_subst_t_lc_t : lngen.
+
+Lemma e_subst_u_lc_u :
+forall u1 u2 x1,
+  lc_u u1 ->
+  lc_u u2 ->
+  lc_u (e_subst_u u2 x1 u1).
+Proof. Admitted.
+
+Hint Resolve e_subst_u_lc_u : lngen.
 
 Lemma t_subst_u_lc_u :
 forall u1 t1 a1,
   lc_u u1 ->
   lc_t t1 ->
   lc_u (t_subst_u t1 a1 u1).
-Proof.
-default_simp.
-Qed.
+Proof. Admitted.
 
 Hint Resolve t_subst_u_lc_u : lngen.
 
@@ -2605,10 +3569,7 @@ Lemma t_subst_t_open_t_wrt_t_rec_mutual :
 (forall t3 t1 t2 a1 n1,
   lc_t t1 ->
   t_subst_t t1 a1 (open_t_wrt_t_rec n1 t2 t3) = open_t_wrt_t_rec n1 (t_subst_t t1 a1 t2) (t_subst_t t1 a1 t3)).
-Proof.
-apply_mutual_ind t_mutind;
-default_simp.
-Qed.
+Proof. Admitted.
 
 (* end hide *)
 
@@ -2618,11 +3579,73 @@ Lemma t_subst_t_open_t_wrt_t_rec :
 forall t3 t1 t2 a1 n1,
   lc_t t1 ->
   t_subst_t t1 a1 (open_t_wrt_t_rec n1 t2 t3) = open_t_wrt_t_rec n1 (t_subst_t t1 a1 t2) (t_subst_t t1 a1 t3).
-Proof.
-pose proof t_subst_t_open_t_wrt_t_rec_mutual as H; intuition eauto.
-Qed.
+Proof. Admitted.
 
 Hint Resolve t_subst_t_open_t_wrt_t_rec : lngen.
+
+(* end hide *)
+
+(* begin hide *)
+
+Lemma e_subst_u_open_u_wrt_u_rec_mutual :
+(forall u3 u1 u2 x1 n1,
+  lc_u u1 ->
+  e_subst_u u1 x1 (open_u_wrt_u_rec n1 u2 u3) = open_u_wrt_u_rec n1 (e_subst_u u1 x1 u2) (e_subst_u u1 x1 u3)).
+Proof. Admitted.
+
+(* end hide *)
+
+(* begin hide *)
+
+Lemma e_subst_u_open_u_wrt_u_rec :
+forall u3 u1 u2 x1 n1,
+  lc_u u1 ->
+  e_subst_u u1 x1 (open_u_wrt_u_rec n1 u2 u3) = open_u_wrt_u_rec n1 (e_subst_u u1 x1 u2) (e_subst_u u1 x1 u3).
+Proof. Admitted.
+
+Hint Resolve e_subst_u_open_u_wrt_u_rec : lngen.
+
+(* end hide *)
+
+(* begin hide *)
+
+Lemma e_subst_u_open_u_wrt_t_rec_mutual :
+(forall u2 u1 t1 x1 n1,
+  lc_u u1 ->
+  e_subst_u u1 x1 (open_u_wrt_t_rec n1 t1 u2) = open_u_wrt_t_rec n1 t1 (e_subst_u u1 x1 u2)).
+Proof. Admitted.
+
+(* end hide *)
+
+(* begin hide *)
+
+Lemma e_subst_u_open_u_wrt_t_rec :
+forall u2 u1 t1 x1 n1,
+  lc_u u1 ->
+  e_subst_u u1 x1 (open_u_wrt_t_rec n1 t1 u2) = open_u_wrt_t_rec n1 t1 (e_subst_u u1 x1 u2).
+Proof. Admitted.
+
+Hint Resolve e_subst_u_open_u_wrt_t_rec : lngen.
+
+(* end hide *)
+
+(* begin hide *)
+
+Lemma t_subst_u_open_u_wrt_u_rec_mutual :
+(forall u2 t1 u1 a1 n1,
+  t_subst_u t1 a1 (open_u_wrt_u_rec n1 u1 u2) = open_u_wrt_u_rec n1 (t_subst_u t1 a1 u1) (t_subst_u t1 a1 u2)).
+Proof. Admitted.
+
+(* end hide *)
+
+(* begin hide *)
+
+Lemma t_subst_u_open_u_wrt_u_rec :
+forall u2 t1 u1 a1 n1,
+  t_subst_u t1 a1 (open_u_wrt_u_rec n1 u1 u2) = open_u_wrt_u_rec n1 (t_subst_u t1 a1 u1) (t_subst_u t1 a1 u2).
+Proof. Admitted.
+
+Hint Resolve t_subst_u_open_u_wrt_u_rec : lngen.
 
 (* end hide *)
 
@@ -2632,10 +3655,7 @@ Lemma t_subst_u_open_u_wrt_t_rec_mutual :
 (forall u1 t1 t2 a1 n1,
   lc_t t1 ->
   t_subst_u t1 a1 (open_u_wrt_t_rec n1 t2 u1) = open_u_wrt_t_rec n1 (t_subst_t t1 a1 t2) (t_subst_u t1 a1 u1)).
-Proof.
-apply_mutual_ind u_mutind;
-default_simp.
-Qed.
+Proof. Admitted.
 
 (* end hide *)
 
@@ -2645,9 +3665,7 @@ Lemma t_subst_u_open_u_wrt_t_rec :
 forall u1 t1 t2 a1 n1,
   lc_t t1 ->
   t_subst_u t1 a1 (open_u_wrt_t_rec n1 t2 u1) = open_u_wrt_t_rec n1 (t_subst_t t1 a1 t2) (t_subst_u t1 a1 u1).
-Proof.
-pose proof t_subst_u_open_u_wrt_t_rec_mutual as H; intuition eauto.
-Qed.
+Proof. Admitted.
 
 Hint Resolve t_subst_u_open_u_wrt_t_rec : lngen.
 
@@ -2657,19 +3675,38 @@ Lemma t_subst_t_open_t_wrt_t :
 forall t3 t1 t2 a1,
   lc_t t1 ->
   t_subst_t t1 a1 (open_t_wrt_t t3 t2) = open_t_wrt_t (t_subst_t t1 a1 t3) (t_subst_t t1 a1 t2).
-Proof.
-unfold open_t_wrt_t; default_simp.
-Qed.
+Proof. Admitted.
 
 Hint Resolve t_subst_t_open_t_wrt_t : lngen.
+
+Lemma e_subst_u_open_u_wrt_u :
+forall u3 u1 u2 x1,
+  lc_u u1 ->
+  e_subst_u u1 x1 (open_u_wrt_u u3 u2) = open_u_wrt_u (e_subst_u u1 x1 u3) (e_subst_u u1 x1 u2).
+Proof. Admitted.
+
+Hint Resolve e_subst_u_open_u_wrt_u : lngen.
+
+Lemma e_subst_u_open_u_wrt_t :
+forall u2 u1 t1 x1,
+  lc_u u1 ->
+  e_subst_u u1 x1 (open_u_wrt_t u2 t1) = open_u_wrt_t (e_subst_u u1 x1 u2) t1.
+Proof. Admitted.
+
+Hint Resolve e_subst_u_open_u_wrt_t : lngen.
+
+Lemma t_subst_u_open_u_wrt_u :
+forall u2 t1 u1 a1,
+  t_subst_u t1 a1 (open_u_wrt_u u2 u1) = open_u_wrt_u (t_subst_u t1 a1 u2) (t_subst_u t1 a1 u1).
+Proof. Admitted.
+
+Hint Resolve t_subst_u_open_u_wrt_u : lngen.
 
 Lemma t_subst_u_open_u_wrt_t :
 forall u1 t1 t2 a1,
   lc_t t1 ->
   t_subst_u t1 a1 (open_u_wrt_t u1 t2) = open_u_wrt_t (t_subst_u t1 a1 u1) (t_subst_t t1 a1 t2).
-Proof.
-unfold open_u_wrt_t; default_simp.
-Qed.
+Proof. Admitted.
 
 Hint Resolve t_subst_u_open_u_wrt_t : lngen.
 
@@ -2678,20 +3715,40 @@ forall t2 t1 a1 a2,
   a1 <> a2 ->
   lc_t t1 ->
   open_t_wrt_t (t_subst_t t1 a1 t2) (t_var_f a2) = t_subst_t t1 a1 (open_t_wrt_t t2 (t_var_f a2)).
-Proof.
-intros; rewrite t_subst_t_open_t_wrt_t; default_simp.
-Qed.
+Proof. Admitted.
 
 Hint Resolve t_subst_t_open_t_wrt_t_var : lngen.
+
+Lemma e_subst_u_open_u_wrt_u_var :
+forall u2 u1 x1 x2,
+  x1 <> x2 ->
+  lc_u u1 ->
+  open_u_wrt_u (e_subst_u u1 x1 u2) (u_var_f x2) = e_subst_u u1 x1 (open_u_wrt_u u2 (u_var_f x2)).
+Proof. Admitted.
+
+Hint Resolve e_subst_u_open_u_wrt_u_var : lngen.
+
+Lemma e_subst_u_open_u_wrt_t_var :
+forall u2 u1 x1 a1,
+  lc_u u1 ->
+  open_u_wrt_t (e_subst_u u1 x1 u2) (t_var_f a1) = e_subst_u u1 x1 (open_u_wrt_t u2 (t_var_f a1)).
+Proof. Admitted.
+
+Hint Resolve e_subst_u_open_u_wrt_t_var : lngen.
+
+Lemma t_subst_u_open_u_wrt_u_var :
+forall u1 t1 a1 x1,
+  open_u_wrt_u (t_subst_u t1 a1 u1) (u_var_f x1) = t_subst_u t1 a1 (open_u_wrt_u u1 (u_var_f x1)).
+Proof. Admitted.
+
+Hint Resolve t_subst_u_open_u_wrt_u_var : lngen.
 
 Lemma t_subst_u_open_u_wrt_t_var :
 forall u1 t1 a1 a2,
   a1 <> a2 ->
   lc_t t1 ->
   open_u_wrt_t (t_subst_u t1 a1 u1) (t_var_f a2) = t_subst_u t1 a1 (open_u_wrt_t u1 (t_var_f a2)).
-Proof.
-intros; rewrite t_subst_u_open_u_wrt_t; default_simp.
-Qed.
+Proof. Admitted.
 
 Hint Resolve t_subst_u_open_u_wrt_t_var : lngen.
 
@@ -2700,10 +3757,7 @@ Hint Resolve t_subst_u_open_u_wrt_t_var : lngen.
 Lemma t_subst_t_spec_rec_mutual :
 (forall t1 t2 a1 n1,
   t_subst_t t2 a1 t1 = open_t_wrt_t_rec n1 t2 (close_t_wrt_t_rec n1 a1 t1)).
-Proof.
-apply_mutual_ind t_mutind;
-default_simp.
-Qed.
+Proof. Admitted.
 
 (* end hide *)
 
@@ -2712,11 +3766,29 @@ Qed.
 Lemma t_subst_t_spec_rec :
 forall t1 t2 a1 n1,
   t_subst_t t2 a1 t1 = open_t_wrt_t_rec n1 t2 (close_t_wrt_t_rec n1 a1 t1).
-Proof.
-pose proof t_subst_t_spec_rec_mutual as H; intuition eauto.
-Qed.
+Proof. Admitted.
 
 Hint Resolve t_subst_t_spec_rec : lngen.
+
+(* end hide *)
+
+(* begin hide *)
+
+Lemma e_subst_u_spec_rec_mutual :
+(forall u1 u2 x1 n1,
+  e_subst_u u2 x1 u1 = open_u_wrt_u_rec n1 u2 (close_u_wrt_u_rec n1 x1 u1)).
+Proof. Admitted.
+
+(* end hide *)
+
+(* begin hide *)
+
+Lemma e_subst_u_spec_rec :
+forall u1 u2 x1 n1,
+  e_subst_u u2 x1 u1 = open_u_wrt_u_rec n1 u2 (close_u_wrt_u_rec n1 x1 u1).
+Proof. Admitted.
+
+Hint Resolve e_subst_u_spec_rec : lngen.
 
 (* end hide *)
 
@@ -2725,10 +3797,7 @@ Hint Resolve t_subst_t_spec_rec : lngen.
 Lemma t_subst_u_spec_rec_mutual :
 (forall u1 t1 a1 n1,
   t_subst_u t1 a1 u1 = open_u_wrt_t_rec n1 t1 (close_u_wrt_t_rec n1 a1 u1)).
-Proof.
-apply_mutual_ind u_mutind;
-default_simp.
-Qed.
+Proof. Admitted.
 
 (* end hide *)
 
@@ -2737,9 +3806,7 @@ Qed.
 Lemma t_subst_u_spec_rec :
 forall u1 t1 a1 n1,
   t_subst_u t1 a1 u1 = open_u_wrt_t_rec n1 t1 (close_u_wrt_t_rec n1 a1 u1).
-Proof.
-pose proof t_subst_u_spec_rec_mutual as H; intuition eauto.
-Qed.
+Proof. Admitted.
 
 Hint Resolve t_subst_u_spec_rec : lngen.
 
@@ -2748,18 +3815,21 @@ Hint Resolve t_subst_u_spec_rec : lngen.
 Lemma t_subst_t_spec :
 forall t1 t2 a1,
   t_subst_t t2 a1 t1 = open_t_wrt_t (close_t_wrt_t a1 t1) t2.
-Proof.
-unfold close_t_wrt_t; unfold open_t_wrt_t; default_simp.
-Qed.
+Proof. Admitted.
 
 Hint Resolve t_subst_t_spec : lngen.
+
+Lemma e_subst_u_spec :
+forall u1 u2 x1,
+  e_subst_u u2 x1 u1 = open_u_wrt_u (close_u_wrt_u x1 u1) u2.
+Proof. Admitted.
+
+Hint Resolve e_subst_u_spec : lngen.
 
 Lemma t_subst_u_spec :
 forall u1 t1 a1,
   t_subst_u t1 a1 u1 = open_u_wrt_t (close_u_wrt_t a1 u1) t1.
-Proof.
-unfold close_u_wrt_t; unfold open_u_wrt_t; default_simp.
-Qed.
+Proof. Admitted.
 
 Hint Resolve t_subst_u_spec : lngen.
 
@@ -2770,10 +3840,7 @@ Lemma t_subst_t_t_subst_t_mutual :
   a2 `notin` tt_fv_t t2 ->
   a2 <> a1 ->
   t_subst_t t2 a1 (t_subst_t t3 a2 t1) = t_subst_t (t_subst_t t2 a1 t3) a2 (t_subst_t t2 a1 t1)).
-Proof.
-apply_mutual_ind t_mutind;
-default_simp.
-Qed.
+Proof. Admitted.
 
 (* end hide *)
 
@@ -2782,11 +3849,63 @@ forall t1 t2 t3 a2 a1,
   a2 `notin` tt_fv_t t2 ->
   a2 <> a1 ->
   t_subst_t t2 a1 (t_subst_t t3 a2 t1) = t_subst_t (t_subst_t t2 a1 t3) a2 (t_subst_t t2 a1 t1).
-Proof.
-pose proof t_subst_t_t_subst_t_mutual as H; intuition eauto.
-Qed.
+Proof. Admitted.
 
 Hint Resolve t_subst_t_t_subst_t : lngen.
+
+(* begin hide *)
+
+Lemma e_subst_u_e_subst_u_mutual :
+(forall u1 u2 u3 x2 x1,
+  x2 `notin` e_fv_u u2 ->
+  x2 <> x1 ->
+  e_subst_u u2 x1 (e_subst_u u3 x2 u1) = e_subst_u (e_subst_u u2 x1 u3) x2 (e_subst_u u2 x1 u1)).
+Proof. Admitted.
+
+(* end hide *)
+
+Lemma e_subst_u_e_subst_u :
+forall u1 u2 u3 x2 x1,
+  x2 `notin` e_fv_u u2 ->
+  x2 <> x1 ->
+  e_subst_u u2 x1 (e_subst_u u3 x2 u1) = e_subst_u (e_subst_u u2 x1 u3) x2 (e_subst_u u2 x1 u1).
+Proof. Admitted.
+
+Hint Resolve e_subst_u_e_subst_u : lngen.
+
+(* begin hide *)
+
+Lemma e_subst_u_t_subst_u_mutual :
+(forall u1 u2 t1 a1 x1,
+  a1 `notin` tt_fv_u u2 ->
+  e_subst_u u2 x1 (t_subst_u t1 a1 u1) = t_subst_u t1 a1 (e_subst_u u2 x1 u1)).
+Proof. Admitted.
+
+(* end hide *)
+
+Lemma e_subst_u_t_subst_u :
+forall u1 u2 t1 a1 x1,
+  a1 `notin` tt_fv_u u2 ->
+  e_subst_u u2 x1 (t_subst_u t1 a1 u1) = t_subst_u t1 a1 (e_subst_u u2 x1 u1).
+Proof. Admitted.
+
+Hint Resolve e_subst_u_t_subst_u : lngen.
+
+(* begin hide *)
+
+Lemma t_subst_u_e_subst_u_mutual :
+(forall u1 t1 u2 x1 a1,
+  t_subst_u t1 a1 (e_subst_u u2 x1 u1) = e_subst_u (t_subst_u t1 a1 u2) x1 (t_subst_u t1 a1 u1)).
+Proof. Admitted.
+
+(* end hide *)
+
+Lemma t_subst_u_e_subst_u :
+forall u1 t1 u2 x1 a1,
+  t_subst_u t1 a1 (e_subst_u u2 x1 u1) = e_subst_u (t_subst_u t1 a1 u2) x1 (t_subst_u t1 a1 u1).
+Proof. Admitted.
+
+Hint Resolve t_subst_u_e_subst_u : lngen.
 
 (* begin hide *)
 
@@ -2795,10 +3914,7 @@ Lemma t_subst_u_t_subst_u_mutual :
   a2 `notin` tt_fv_t t1 ->
   a2 <> a1 ->
   t_subst_u t1 a1 (t_subst_u t2 a2 u1) = t_subst_u (t_subst_t t1 a1 t2) a2 (t_subst_u t1 a1 u1)).
-Proof.
-apply_mutual_ind u_mutind;
-default_simp.
-Qed.
+Proof. Admitted.
 
 (* end hide *)
 
@@ -2807,9 +3923,7 @@ forall u1 t1 t2 a2 a1,
   a2 `notin` tt_fv_t t1 ->
   a2 <> a1 ->
   t_subst_u t1 a1 (t_subst_u t2 a2 u1) = t_subst_u (t_subst_t t1 a1 t2) a2 (t_subst_u t1 a1 u1).
-Proof.
-pose proof t_subst_u_t_subst_u_mutual as H; intuition eauto.
-Qed.
+Proof. Admitted.
 
 Hint Resolve t_subst_u_t_subst_u : lngen.
 
@@ -2822,10 +3936,7 @@ Lemma t_subst_t_close_t_wrt_t_rec_open_t_wrt_t_rec_mutual :
   a2 <> a1 ->
   degree_t_wrt_t n1 t1 ->
   t_subst_t t1 a1 t2 = close_t_wrt_t_rec n1 a2 (t_subst_t t1 a1 (open_t_wrt_t_rec n1 (t_var_f a2) t2))).
-Proof.
-apply_mutual_ind t_mutrec;
-default_simp.
-Qed.
+Proof. Admitted.
 
 (* end hide *)
 
@@ -2838,11 +3949,85 @@ forall t2 t1 a1 a2 n1,
   a2 <> a1 ->
   degree_t_wrt_t n1 t1 ->
   t_subst_t t1 a1 t2 = close_t_wrt_t_rec n1 a2 (t_subst_t t1 a1 (open_t_wrt_t_rec n1 (t_var_f a2) t2)).
-Proof.
-pose proof t_subst_t_close_t_wrt_t_rec_open_t_wrt_t_rec_mutual as H; intuition eauto.
-Qed.
+Proof. Admitted.
 
 Hint Resolve t_subst_t_close_t_wrt_t_rec_open_t_wrt_t_rec : lngen.
+
+(* end hide *)
+
+(* begin hide *)
+
+Lemma e_subst_u_close_u_wrt_u_rec_open_u_wrt_u_rec_mutual :
+(forall u2 u1 x1 x2 n1,
+  x2 `notin` e_fv_u u2 ->
+  x2 `notin` e_fv_u u1 ->
+  x2 <> x1 ->
+  degree_u_wrt_u n1 u1 ->
+  e_subst_u u1 x1 u2 = close_u_wrt_u_rec n1 x2 (e_subst_u u1 x1 (open_u_wrt_u_rec n1 (u_var_f x2) u2))).
+Proof. Admitted.
+
+(* end hide *)
+
+(* begin hide *)
+
+Lemma e_subst_u_close_u_wrt_u_rec_open_u_wrt_u_rec :
+forall u2 u1 x1 x2 n1,
+  x2 `notin` e_fv_u u2 ->
+  x2 `notin` e_fv_u u1 ->
+  x2 <> x1 ->
+  degree_u_wrt_u n1 u1 ->
+  e_subst_u u1 x1 u2 = close_u_wrt_u_rec n1 x2 (e_subst_u u1 x1 (open_u_wrt_u_rec n1 (u_var_f x2) u2)).
+Proof. Admitted.
+
+Hint Resolve e_subst_u_close_u_wrt_u_rec_open_u_wrt_u_rec : lngen.
+
+(* end hide *)
+
+(* begin hide *)
+
+Lemma e_subst_u_close_u_wrt_t_rec_open_u_wrt_t_rec_mutual :
+(forall u2 u1 x1 a1 n1,
+  a1 `notin` tt_fv_u u2 ->
+  a1 `notin` tt_fv_u u1 ->
+  degree_u_wrt_t n1 u1 ->
+  e_subst_u u1 x1 u2 = close_u_wrt_t_rec n1 a1 (e_subst_u u1 x1 (open_u_wrt_t_rec n1 (t_var_f a1) u2))).
+Proof. Admitted.
+
+(* end hide *)
+
+(* begin hide *)
+
+Lemma e_subst_u_close_u_wrt_t_rec_open_u_wrt_t_rec :
+forall u2 u1 x1 a1 n1,
+  a1 `notin` tt_fv_u u2 ->
+  a1 `notin` tt_fv_u u1 ->
+  degree_u_wrt_t n1 u1 ->
+  e_subst_u u1 x1 u2 = close_u_wrt_t_rec n1 a1 (e_subst_u u1 x1 (open_u_wrt_t_rec n1 (t_var_f a1) u2)).
+Proof. Admitted.
+
+Hint Resolve e_subst_u_close_u_wrt_t_rec_open_u_wrt_t_rec : lngen.
+
+(* end hide *)
+
+(* begin hide *)
+
+Lemma t_subst_u_close_u_wrt_u_rec_open_u_wrt_u_rec_mutual :
+(forall u1 t1 a1 x1 n1,
+  x1 `notin` e_fv_u u1 ->
+  t_subst_u t1 a1 u1 = close_u_wrt_u_rec n1 x1 (t_subst_u t1 a1 (open_u_wrt_u_rec n1 (u_var_f x1) u1))).
+Proof. Admitted.
+
+(* end hide *)
+
+(* begin hide *)
+
+Lemma t_subst_u_close_u_wrt_u_rec_open_u_wrt_u_rec :
+forall u1 t1 a1 x1 n1,
+  x1 `notin` e_fv_u u1 ->
+  t_subst_u t1 a1 u1 = close_u_wrt_u_rec n1 x1 (t_subst_u t1 a1 (open_u_wrt_u_rec n1 (u_var_f x1) u1)).
+Proof. Admitted.
+
+Hint Resolve t_subst_u_close_u_wrt_u_rec_open_u_wrt_u_rec : lngen.
 
 (* end hide *)
 
@@ -2855,10 +4040,7 @@ Lemma t_subst_u_close_u_wrt_t_rec_open_u_wrt_t_rec_mutual :
   a2 <> a1 ->
   degree_t_wrt_t n1 t1 ->
   t_subst_u t1 a1 u1 = close_u_wrt_t_rec n1 a2 (t_subst_u t1 a1 (open_u_wrt_t_rec n1 (t_var_f a2) u1))).
-Proof.
-apply_mutual_ind u_mutrec;
-default_simp.
-Qed.
+Proof. Admitted.
 
 (* end hide *)
 
@@ -2871,9 +4053,7 @@ forall u1 t1 a1 a2 n1,
   a2 <> a1 ->
   degree_t_wrt_t n1 t1 ->
   t_subst_u t1 a1 u1 = close_u_wrt_t_rec n1 a2 (t_subst_u t1 a1 (open_u_wrt_t_rec n1 (t_var_f a2) u1)).
-Proof.
-pose proof t_subst_u_close_u_wrt_t_rec_open_u_wrt_t_rec_mutual as H; intuition eauto.
-Qed.
+Proof. Admitted.
 
 Hint Resolve t_subst_u_close_u_wrt_t_rec_open_u_wrt_t_rec : lngen.
 
@@ -2886,11 +4066,39 @@ forall t2 t1 a1 a2,
   a2 <> a1 ->
   lc_t t1 ->
   t_subst_t t1 a1 t2 = close_t_wrt_t a2 (t_subst_t t1 a1 (open_t_wrt_t t2 (t_var_f a2))).
-Proof.
-unfold close_t_wrt_t; unfold open_t_wrt_t; default_simp.
-Qed.
+Proof. Admitted.
 
 Hint Resolve t_subst_t_close_t_wrt_t_open_t_wrt_t : lngen.
+
+Lemma e_subst_u_close_u_wrt_u_open_u_wrt_u :
+forall u2 u1 x1 x2,
+  x2 `notin` e_fv_u u2 ->
+  x2 `notin` e_fv_u u1 ->
+  x2 <> x1 ->
+  lc_u u1 ->
+  e_subst_u u1 x1 u2 = close_u_wrt_u x2 (e_subst_u u1 x1 (open_u_wrt_u u2 (u_var_f x2))).
+Proof. Admitted.
+
+Hint Resolve e_subst_u_close_u_wrt_u_open_u_wrt_u : lngen.
+
+Lemma e_subst_u_close_u_wrt_t_open_u_wrt_t :
+forall u2 u1 x1 a1,
+  a1 `notin` tt_fv_u u2 ->
+  a1 `notin` tt_fv_u u1 ->
+  lc_u u1 ->
+  e_subst_u u1 x1 u2 = close_u_wrt_t a1 (e_subst_u u1 x1 (open_u_wrt_t u2 (t_var_f a1))).
+Proof. Admitted.
+
+Hint Resolve e_subst_u_close_u_wrt_t_open_u_wrt_t : lngen.
+
+Lemma t_subst_u_close_u_wrt_u_open_u_wrt_u :
+forall u1 t1 a1 x1,
+  x1 `notin` e_fv_u u1 ->
+  lc_t t1 ->
+  t_subst_u t1 a1 u1 = close_u_wrt_u x1 (t_subst_u t1 a1 (open_u_wrt_u u1 (u_var_f x1))).
+Proof. Admitted.
+
+Hint Resolve t_subst_u_close_u_wrt_u_open_u_wrt_u : lngen.
 
 Lemma t_subst_u_close_u_wrt_t_open_u_wrt_t :
 forall u1 t1 a1 a2,
@@ -2899,9 +4107,7 @@ forall u1 t1 a1 a2,
   a2 <> a1 ->
   lc_t t1 ->
   t_subst_u t1 a1 u1 = close_u_wrt_t a2 (t_subst_u t1 a1 (open_u_wrt_t u1 (t_var_f a2))).
-Proof.
-unfold close_u_wrt_t; unfold open_u_wrt_t; default_simp.
-Qed.
+Proof. Admitted.
 
 Hint Resolve t_subst_u_close_u_wrt_t_open_u_wrt_t : lngen.
 
@@ -2910,20 +4116,61 @@ forall a2 t2 t1 a1,
   lc_t t1 ->
   a2 `notin` tt_fv_t t1 `union` tt_fv_t t2 `union` singleton a1 ->
   t_subst_t t1 a1 (t_all t2) = t_all (close_t_wrt_t a2 (t_subst_t t1 a1 (open_t_wrt_t t2 (t_var_f a2)))).
-Proof.
-default_simp.
-Qed.
+Proof. Admitted.
 
 Hint Resolve t_subst_t_t_all : lngen.
+
+Lemma e_subst_u_u_fix :
+forall x2 t1 t2 e1 u1 x1,
+  lc_u u1 ->
+  x2 `notin` e_fv_u u1 `union` e_fv_u e1 `union` singleton x1 ->
+  e_subst_u u1 x1 (u_fix t1 t2 e1) = u_fix (t1) (t2) (close_u_wrt_u x2 (e_subst_u u1 x1 (open_u_wrt_u e1 (u_var_f x2)))).
+Proof. Admitted.
+
+Hint Resolve e_subst_u_u_fix : lngen.
+
+Lemma e_subst_u_u_lam :
+forall x2 t1 e1 u1 x1,
+  lc_u u1 ->
+  x2 `notin` e_fv_u u1 `union` e_fv_u e1 `union` singleton x1 ->
+  e_subst_u u1 x1 (u_lam t1 e1) = u_lam (t1) (close_u_wrt_u x2 (e_subst_u u1 x1 (open_u_wrt_u e1 (u_var_f x2)))).
+Proof. Admitted.
+
+Hint Resolve e_subst_u_u_lam : lngen.
+
+Lemma e_subst_u_u_tlam :
+forall a1 e1 u1 x1,
+  lc_u u1 ->
+  a1 `notin` tt_fv_u u1 `union` tt_fv_u e1 ->
+  e_subst_u u1 x1 (u_tlam e1) = u_tlam (close_u_wrt_t a1 (e_subst_u u1 x1 (open_u_wrt_t e1 (t_var_f a1)))).
+Proof. Admitted.
+
+Hint Resolve e_subst_u_u_tlam : lngen.
+
+Lemma t_subst_u_u_fix :
+forall x1 t2 t3 e1 t1 a1,
+  lc_t t1 ->
+  x1 `notin` e_fv_u e1 ->
+  t_subst_u t1 a1 (u_fix t2 t3 e1) = u_fix (t_subst_t t1 a1 t2) (t_subst_t t1 a1 t3) (close_u_wrt_u x1 (t_subst_u t1 a1 (open_u_wrt_u e1 (u_var_f x1)))).
+Proof. Admitted.
+
+Hint Resolve t_subst_u_u_fix : lngen.
+
+Lemma t_subst_u_u_lam :
+forall x1 t2 e1 t1 a1,
+  lc_t t1 ->
+  x1 `notin` e_fv_u e1 ->
+  t_subst_u t1 a1 (u_lam t2 e1) = u_lam (t_subst_t t1 a1 t2) (close_u_wrt_u x1 (t_subst_u t1 a1 (open_u_wrt_u e1 (u_var_f x1)))).
+Proof. Admitted.
+
+Hint Resolve t_subst_u_u_lam : lngen.
 
 Lemma t_subst_u_u_tlam :
 forall a2 e1 t1 a1,
   lc_t t1 ->
   a2 `notin` tt_fv_t t1 `union` tt_fv_u e1 `union` singleton a1 ->
   t_subst_u t1 a1 (u_tlam e1) = u_tlam (close_u_wrt_t a2 (t_subst_u t1 a1 (open_u_wrt_t e1 (t_var_f a2)))).
-Proof.
-default_simp.
-Qed.
+Proof. Admitted.
 
 Hint Resolve t_subst_u_u_tlam : lngen.
 
@@ -2933,10 +4180,7 @@ Lemma t_subst_t_intro_rec_mutual :
 (forall t1 a1 t2 n1,
   a1 `notin` tt_fv_t t1 ->
   open_t_wrt_t_rec n1 t2 t1 = t_subst_t t2 a1 (open_t_wrt_t_rec n1 (t_var_f a1) t1)).
-Proof.
-apply_mutual_ind t_mutind;
-default_simp.
-Qed.
+Proof. Admitted.
 
 (* end hide *)
 
@@ -2944,12 +4188,29 @@ Lemma t_subst_t_intro_rec :
 forall t1 a1 t2 n1,
   a1 `notin` tt_fv_t t1 ->
   open_t_wrt_t_rec n1 t2 t1 = t_subst_t t2 a1 (open_t_wrt_t_rec n1 (t_var_f a1) t1).
-Proof.
-pose proof t_subst_t_intro_rec_mutual as H; intuition eauto.
-Qed.
+Proof. Admitted.
 
 Hint Resolve t_subst_t_intro_rec : lngen.
 Hint Rewrite t_subst_t_intro_rec using solve [auto] : lngen.
+
+(* begin hide *)
+
+Lemma e_subst_u_intro_rec_mutual :
+(forall u1 x1 u2 n1,
+  x1 `notin` e_fv_u u1 ->
+  open_u_wrt_u_rec n1 u2 u1 = e_subst_u u2 x1 (open_u_wrt_u_rec n1 (u_var_f x1) u1)).
+Proof. Admitted.
+
+(* end hide *)
+
+Lemma e_subst_u_intro_rec :
+forall u1 x1 u2 n1,
+  x1 `notin` e_fv_u u1 ->
+  open_u_wrt_u_rec n1 u2 u1 = e_subst_u u2 x1 (open_u_wrt_u_rec n1 (u_var_f x1) u1).
+Proof. Admitted.
+
+Hint Resolve e_subst_u_intro_rec : lngen.
+Hint Rewrite e_subst_u_intro_rec using solve [auto] : lngen.
 
 (* begin hide *)
 
@@ -2957,10 +4218,7 @@ Lemma t_subst_u_intro_rec_mutual :
 (forall u1 a1 t1 n1,
   a1 `notin` tt_fv_u u1 ->
   open_u_wrt_t_rec n1 t1 u1 = t_subst_u t1 a1 (open_u_wrt_t_rec n1 (t_var_f a1) u1)).
-Proof.
-apply_mutual_ind u_mutind;
-default_simp.
-Qed.
+Proof. Admitted.
 
 (* end hide *)
 
@@ -2968,9 +4226,7 @@ Lemma t_subst_u_intro_rec :
 forall u1 a1 t1 n1,
   a1 `notin` tt_fv_u u1 ->
   open_u_wrt_t_rec n1 t1 u1 = t_subst_u t1 a1 (open_u_wrt_t_rec n1 (t_var_f a1) u1).
-Proof.
-pose proof t_subst_u_intro_rec_mutual as H; intuition eauto.
-Qed.
+Proof. Admitted.
 
 Hint Resolve t_subst_u_intro_rec : lngen.
 Hint Rewrite t_subst_u_intro_rec using solve [auto] : lngen.
@@ -2979,19 +4235,23 @@ Lemma t_subst_t_intro :
 forall a1 t1 t2,
   a1 `notin` tt_fv_t t1 ->
   open_t_wrt_t t1 t2 = t_subst_t t2 a1 (open_t_wrt_t t1 (t_var_f a1)).
-Proof.
-unfold open_t_wrt_t; default_simp.
-Qed.
+Proof. Admitted.
 
 Hint Resolve t_subst_t_intro : lngen.
+
+Lemma e_subst_u_intro :
+forall x1 u1 u2,
+  x1 `notin` e_fv_u u1 ->
+  open_u_wrt_u u1 u2 = e_subst_u u2 x1 (open_u_wrt_u u1 (u_var_f x1)).
+Proof. Admitted.
+
+Hint Resolve e_subst_u_intro : lngen.
 
 Lemma t_subst_u_intro :
 forall a1 u1 t1,
   a1 `notin` tt_fv_u u1 ->
   open_u_wrt_t u1 t1 = t_subst_u t1 a1 (open_u_wrt_t u1 (t_var_f a1)).
-Proof.
-unfold open_u_wrt_t; default_simp.
-Qed.
+Proof. Admitted.
 
 Hint Resolve t_subst_u_intro : lngen.
 
